Updated cps.v and eval.v to correspond to the new syntax and semantics. Fixed most of the L6 related files including the closure conversion and hoisting transformations and proofs.

theories/L6_PCPS/cps.v
@@ -1,14 +1,15 @@
 (* Continuation-Passing Style language for the CertiCoq project.
  *   Initial design, Andrew W. Appel, June 2014
  *)
-Require Import Coq.Relations.Relations Coq.ZArith.ZArith Coq.ZArith.Znumtheory
-               Coq.Bool.Bool Coq.Lists.List Coq.funind.Recdef.
-Require Import ExtLib.Structures.Monad ExtLib.Core.Type.
-Require Maps.
-Import Nnat.
-
+Require Import Coq.ZArith.ZArith Coq.Lists.List.
+Require Import ExtLib.Structures.Monads ExtLib.Data.Monads.StateMonad.
 Require Import List_util.
-Require Import HashMap.
+
+Require Maps.
+
+Import MonadNotation.
+
+Open Scope monad_scope.
 
 
 (* We will use several maps from identifiers to types, values, etc.
@@ -17,7 +18,6 @@ Require Import HashMap.
  * created, we'll use that. *)
 
 Module M := Maps.PTree.
-Module T := ExtLib.Core.Type.
 
 Fixpoint getlist {A} (xs: list M.elt) (rho: M.t A) : option (list A) :=
   match xs with 
@@ -39,9 +39,11 @@ Fixpoint setlist {A} (xs: list M.elt) (vs: list A) (rho: M.t A) : option (M.t A)
   end.
 
 Definition var := M.elt.   (* value variables *)
-Definition type := positive.
-Definition tag := M.elt.   (* discrimination tags *)
+Definition fTag := M.elt.   (* discrimination tags for functions *)
+Definition iTag := M.elt.   (* discrimination tags for inductive types *)
+Definition cTag := M.elt.   (* discrimination tags for constructors *)
 Definition prim := M.elt. (* primitive operators *)
+
 
 (* Remark.  It sure would be nice if we could use abstraction here,
    so that M was instantiated differently for vars, types, and tags,
@@ -59,8 +61,9 @@ Definition prim := M.elt. (* primitive operators *)
    abstract syntax trees.
  *)
 
+
 (* Given a list of tagged variants, return the one with the matching tag. *)
-Fixpoint findtag {A} (cl: list (tag * A)) (c: tag) : option A :=
+Fixpoint findtag {A} (cl: list (cTag * A)) (c: cTag) : option A :=
   match cl with
     | (c',a)::cl' => if M.elt_eq c' c then Some a else findtag cl' c
     | nil => None
@@ -70,17 +73,15 @@ Fixpoint findtag {A} (cl: list (tag * A)) (c: tag) : option A :=
 
 (* Expressions [exp] of the CPS language. *)
 Inductive exp : Type :=
-| Econstr: var -> type -> tag -> list var -> exp -> exp
-| Ecase: var -> list (tag * exp) -> exp
-| Eproj: var -> type -> N -> var -> exp -> exp
+| Econstr: var -> cTag -> list var -> exp -> exp
+| Ecase: var -> list (cTag * exp) -> exp
+| Eproj: var -> cTag -> N -> var -> exp -> exp
 | Efun: fundefs -> exp -> exp
-| Eapp: var -> list var -> exp
-| Eprim: var -> type -> prim -> list var -> exp -> exp (* where prim is id *)
-(* | Eprim: var -> type -> list var -> exp -> exp *)
+| Eapp: var -> fTag -> list var -> exp
+| Eprim: var -> prim -> list var -> exp -> exp (* where prim is id *)
 with fundefs : Type :=
-     | Fcons: var -> type -> list var -> exp -> fundefs -> fundefs
+     | Fcons: var -> fTag -> list var -> exp -> fundefs -> fundefs
      | Fnil: fundefs.
-
 
 
 (* [Econstr x t c ys e] applies a data constructor with tag [c] to
@@ -127,20 +128,21 @@ with fundefs : Type :=
    (optimization, rewrite) algorithms may require it.
  *)
 
+
 (** Induction principles for exp *)
 Lemma exp_ind' :
   forall P : exp -> Type,
-    (forall (v : var) (t : type) (t0 : tag) (l : list var) (e : exp),
-       P e -> P (Econstr v t t0 l e)) ->
+    (forall (v : var) (t : cTag) (l : list var) (e : exp),
+       P e -> P (Econstr v t l e)) ->
     (forall (v : var), P (Ecase v nil)) ->
-    (forall (v : var) (l : list (tag * exp)) (c : tag) (e : exp),
+    (forall (v : var) (l : list (cTag * exp)) (c : cTag) (e : exp),
        P e -> P (Ecase v l) -> P (Ecase v ((c, e) :: l))) ->
-    (forall (v : var) (t : type) (n : N) (v0 : var) (e : exp),
+    (forall (v : var) (t : cTag) (n : N) (v0 : var) (e : exp),
        P e -> P (Eproj v t n v0 e)) ->
     (forall (f2 : fundefs) (e : exp), P e -> P (Efun f2 e)) ->
-    (forall (v : var) (l : list var), P (Eapp v l)) ->
-    (forall (v : var) (t : type) (p : prim) (l : list var) (e : exp),
-       P e -> P (Eprim v t p l e)) -> forall e : exp, P e.
+    (forall (v : var) (t : fTag) (l : list var), P (Eapp v t l)) ->
+    (forall (v : var)  (p : prim) (l : list var) (e : exp),
+       P e -> P (Eprim v p l e)) -> forall e : exp, P e.
 Proof.
   intros P H1 H2 H3 H4 H5 H6 H7. fix 1.
   destruct e; try (now clear exp_ind'; eauto).
@@ -156,34 +158,34 @@ Qed.
 (** Mutual induction scheme for exp and fundefs *)
 Lemma exp_mut :
   forall (P : exp -> Type) (P0 : fundefs -> Type),
-    (forall (v : var) (t : type) (t0 : tag) (l : list var) (e : exp),
-       P e -> P (Econstr v t t0 l e)) ->
+    (forall (v : var) (t : cTag) (l : list var) (e : exp),
+       P e -> P (Econstr v t l e)) ->
     (forall (v : var), P (Ecase v nil)) ->
-    (forall (v : var) (l : list (tag * exp)) (c : tag) (e : exp),
+    (forall (v : var) (l : list (cTag * exp)) (c : cTag) (e : exp),
        P e -> P (Ecase v l) -> P (Ecase v ((c, e) :: l))) ->
-    (forall (v : var) (t : type) (n : N) (v0 : var) (e : exp),
+    (forall (v : var) (t : cTag) (n : N) (v0 : var) (e : exp),
        P e -> P (Eproj v t n v0 e)) ->
     (forall f2 : fundefs, P0 f2 -> forall e : exp, P e -> P (Efun f2 e)) ->
-    (forall (v : var) (l : list var), P (Eapp v l)) ->
-    (forall (v : var) (t : type) (p : prim) (l : list var) (e : exp),
-       P e -> P (Eprim v t p l e)) ->
-    (forall (v : var) (t : type) (l : list var) (e : exp),
+    (forall (v : var) (t : fTag) (l : list var), P (Eapp v t l)) ->
+    (forall (v : var) (p : prim) (l : list var) (e : exp),
+       P e -> P (Eprim v p l e)) ->
+    (forall (v : var) (t : fTag) (l : list var) (e : exp),
        P e -> forall f5 : fundefs, P0 f5 -> P0 (Fcons v t l e f5)) ->
     P0 Fnil -> forall e : exp, P e                                 
 with fundefs_mut :
   forall (P : exp -> Type) (P0 : fundefs -> Type),
-    (forall (v : var) (t : type) (t0 : tag) (l : list var) (e : exp),
-       P e -> P (Econstr v t t0 l e)) ->
+    (forall (v : var) (t : cTag) (l : list var) (e : exp),
+       P e -> P (Econstr v t l e)) ->
     (forall (v : var), P (Ecase v nil)) ->
-    (forall (v : var) (l : list (tag * exp)) (c : tag) (e : exp),
+    (forall (v : var) (l : list (cTag * exp)) (c : cTag) (e : exp),
        P e -> P (Ecase v l) -> P (Ecase v ((c, e) :: l))) ->
-    (forall (v : var) (t : type) (n : N) (v0 : var) (e : exp),
+    (forall (v : var) (t : cTag) (n : N) (v0 : var) (e : exp),
        P e -> P (Eproj v t n v0 e)) ->
     (forall f2 : fundefs, P0 f2 -> forall e : exp, P e -> P (Efun f2 e)) ->
-    (forall (v : var) (l : list var), P (Eapp v l)) ->
-    (forall (v : var) (t : type) (p : prim) (l : list var) (e : exp),
-       P e -> P (Eprim v t p l e)) ->
-    (forall (v : var) (t : type) (l : list var) (e : exp),
+    (forall (v : var) (t : fTag) (l : list var), P (Eapp v t l)) ->
+    (forall (v : var) (p : prim) (l : list var) (e : exp),
+       P e -> P (Eprim v p l e)) ->
+    (forall (v : var) (t : fTag) (l : list var) (e : exp),
        P e -> forall f5 : fundefs, P0 f5 -> P0 (Fcons v t l e f5)) ->
     P0 Fnil -> forall f7 : fundefs, P0 f7.
 Proof.
@@ -206,18 +208,18 @@ Qed.
 (* to do proofs simultaneously. *)
 Lemma exp_def_mutual_ind :
   forall (P : exp -> Prop) (P0 : fundefs -> Prop),
-    (forall (v : var) (t : type) (t0 : tag) (l : list var) (e : exp),
-       P e -> P (Econstr v t t0 l e)) ->
+    (forall (v : var) (t : cTag) (l : list var) (e : exp),
+       P e -> P (Econstr v t l e)) ->
     (forall (v : var), P (Ecase v nil)) ->
-    (forall (v : var) (l : list (tag * exp)) (c : tag) (e : exp),
+    (forall (v : var) (l : list (cTag * exp)) (c : cTag) (e : exp),
        P e -> P (Ecase v l) -> P (Ecase v ((c, e) :: l))) ->
-    (forall (v : var) (t : type) (n : N) (v0 : var) (e : exp),
+    (forall (v : var) (t : cTag) (n : N) (v0 : var) (e : exp),
        P e -> P (Eproj v t n v0 e)) ->
     (forall f2 : fundefs, P0 f2 -> forall e : exp, P e -> P (Efun f2 e)) ->
-    (forall (v : var) (l : list var), P (Eapp v l)) ->
-    (forall (v : var) (t : type) (p : prim) (l : list var) (e : exp),
-       P e -> P (Eprim v t p l e)) ->
-    (forall (v : var) (t : type) (l : list var) (e : exp),
+    (forall (v : var) (t : fTag) (l : list var), P (Eapp v t l)) ->
+    (forall (v : var) (p : prim) (l : list var) (e : exp),
+       P e -> P (Eprim v p l e)) ->
+    (forall (v : var) (t : fTag) (l : list var) (e : exp),
        P e -> forall f5 : fundefs, P0 f5 -> P0 (Fcons v t l e f5)) ->
     P0 Fnil -> (forall e : exp, P e) /\ (forall f : fundefs, P0 f).
 Proof.
@@ -226,36 +228,37 @@ Proof.
   apply (fundefs_mut P P0); assumption.
 Qed.
 
+
 (** name the induction hypotheses only *)
 Ltac exp_defs_induction IH1 IHl IH2 :=
   apply exp_def_mutual_ind;
-  [ intros ? ? ? ? ? IH1 
+  [ intros ? ? ? ? IH1 
   | intros ?
   | intros ? ? ? ? IH1 IHl 
   | intros ? ? ? ? ? IH1
   | intros ? IH2 ? IH1 
-  | intros ? ?
-  | intros ? ? ? ? ? IH1 
+  | intros ? ? ?
+  | intros ? ? ? ? IH1 
   | intros ? ? ? ? IH1 ? IH2
   | ].
 
 (** * CPS Values *)
 
 Inductive val : Type :=
-| Vconstr: type -> tag -> list val -> val
+| Vconstr: cTag -> list val -> val
 | Vfun: M.t val -> fundefs -> var -> val
-(* Vfun env fds f where 
-       env is the environment at the function binding site
-       fds is the list of mutually recursive functions including f *)
+(* [Vfun env fds f]
+     where env is the environment at the function binding site
+     fds is the list of mutually recursive functions including f *)
 | Vint: Z -> val.
 
 
 (** Induction principle for values. *)
 Lemma val_ind' :
   forall P : val -> Prop,
-    (forall (tau : type) (t : tag), P (Vconstr tau t nil)) ->
-    (forall (tau : type) (t : tag) (v : val) (l : list val),
-       P v -> P (Vconstr tau t l) -> P (Vconstr tau t (v :: l))) ->
+    (forall (t : cTag), P (Vconstr t nil)) ->
+    (forall (t : cTag) (v : val) (l : list val),
+       P v -> P (Vconstr t l) -> P (Vconstr t (v :: l))) ->
     (forall (t : M.t val) (f0 : fundefs) (v : var), P (Vfun t f0 v)) ->
     (forall z : Z, P (Vint z)) ->
     forall v : val, P v.
@@ -280,262 +283,56 @@ Fixpoint find_def (f: var) (fl:  fundefs) :=
     | Fnil => None
   end.
 
+(*********** type info ********************)
+(* Will probably be updated to be a HashMap to get fresh tags instead of state *)
 
-  (** The following are not used anywhere. They have to do either with "well-typedness"
-    * or observable values. We need to go through them to decide if can can through them
-    * away altogether. *)
+(* info of a constructor. Includes: iTag of corresponding inductive type
+                                    the constructor's arity
+                                    the cTags ordinal in inductive defn starting at zero *)
 
-(*********** static typing ******************)
-Inductive typeinfo : Type :=
-| Tdata: list (tag * list type) -> typeinfo
-| Tfun: tag -> list type -> typeinfo
-| Tother: tag -> typeinfo
-| Tunknown.
+Definition cTyInfo : Type := iTag * N * N.
 
-(* [Tdata (c1 ts1 :: c2 ts2 :: ... )] is a sum-of-products type.
-   Each disjunct is tagged with a tag ([c1],[c2],...).   No two disjuncts
-   may have the same tag, though the same tag may be used in
-   different data types.  Each disjunct is a product (tuple) of 
-   fields, with types given by the list [ts].  A tag may stand for any
-   of many possible concrete representation strategies.
+Definition unkownTyInfo : cTyInfo := (1%positive, 0%N, 0%N).
 
-  [Tfun c ts]   is a (continuation) function that takes [length ts] arguments
-    of types [ts] and does not return.  The calling sequence is implied
-    by the tag [c]; function types with different tags are incompatible
-    and never subtype.
+Definition cEnv := M.t cTyInfo.  (* An constructor enironment maps [cTag]s to their information *)
 
-  [Tother c]  allows room for expansion.
- *)
-Require Coq.Structures.Orders.
-Import RelationClasses.
+(* state of next fresh [cTag], [iTag], and the current environment *)
+Definition cState := state (cTag * iTag * cEnv).
 
-(* Demonstrate that typeinfo has a computational total order,
-   so that we can make a HashMap over it. *)
-Module TypeInfo <: Orders.UsualOrderedType.
-  Definition t := typeinfo.
-  Definition eq := @eq t.
-  Definition eq_equiv : Equivalence eq := eq_equivalence.
+(** Get a new cTag *)
+Definition get_cTag : cState cTag :=
+  p <- get ;;
+  let '(n, m, e) := p in
+  put ((n+1)%positive, m, e) ;;
+  ret n.
 
-  Definition lexi {A}{B} (f: A -> A -> comparison) a a' (g: B -> B -> comparison) b b' : comparison :=
-    match f a a' with Lt => Lt | Eq => g b b' | Gt => Gt end.
+(** Get a new iTag *)
+Definition get_iTag : cState iTag :=
+  p <- get ;;
+  let '(n, m, e) := p in
+  put (n,(m+1)%positive, e) ;;
+  ret m.
 
-  Fixpoint compare_list {A} (f: A -> A -> comparison) (al bl: list A) : comparison := 
-    match al, bl with
-      | a::al', b::bl' => lexi f a b (compare_list f) al' bl'
-      | nil, _::_ => Lt
-      | _::_, nil => Gt
-      | nil, nil => Eq
-    end.
+(** set the cTyInfo for a given cTag *)
+Definition set_cTyInfo (x : cTag) (t : cTyInfo) : cState cTag :=
+  p <- get ;;
+  let '(n, m, e) := p in
+  put (n, m, M.set x t e) ;;
+  ret x.
 
-  Fixpoint compare_pair {A}{B} (f: A -> A -> comparison) (g: B -> B -> comparison)
-           (x: A*B) (y: A*B) : comparison :=
-    lexi f (fst x) (fst y) g (snd x) (snd y).
-
-  Fixpoint compare (x y : t) : comparison :=
-    match x, y with
-      | Tdata tl, Tdata tl' => 
-        compare_list (compare_pair Pos.compare (compare_list Pos.compare)) tl tl'
-      | Tdata _, _ => Lt
-      | _, Tdata _ => Gt
-      | Tfun c tl, Tfun c' tl' => lexi Pos.compare c c' (compare_list Pos.compare) tl tl'
-      | Tfun _ _, _ => Lt
-      | _, Tfun _ _ => Gt
-      | Tunknown, _ => Lt
-      | _, Tunknown => Gt
-      | Tother c, Tother c' => Pos.compare c c'
-    end.
-
-  Definition lt (x y: t) : Prop := compare x y = Lt.
-  Lemma lt_strorder: StrictOrder lt.
-  Proof.
-  Admitted.
-
-  Lemma lt_compat:  Morphisms.Proper
-                      (Morphisms.respectful Logic.eq (Morphisms.respectful Logic.eq iff)) lt.
-  Proof.
-    hnf; intros. subst. split; subst; auto.
-  Qed.
-
-  Lemma compare_spec :
-    forall x y : t, CompareSpec (x = y) (lt x y) (lt y x) (compare x y).
-  Proof.
-    intros.
-    destruct (compare x y) eqn:?H;  constructor.
-    admit.
-    auto.
-    admit.
-  Admitted.
-
-  Lemma eq_dec : forall x y : t, {x = y} + {x <> y}.
-  Proof.
-    intros.
-    pose proof (compare_spec x y).
-    destruct (compare x y).
-    left; inversion H; auto.
-    right; inversion H; intro; subst y; destruct (lt_strorder) as [H2 _]. apply (H2 x); auto.
-    right; inversion H; intro; subst y; destruct (lt_strorder) as [H2 _]. apply (H2 x); auto.
-  Defined.
-End TypeInfo.
-
-Module TDict := HashMap.MakeHashMap TypeInfo.
-Definition tdict := TDict.t.
-(* mapping from type to typeinfo.
-   We use a HashMap for this, so that for any typeinfo we can
-   find its (unique) index (i.e., "type"), and for any type we can
-   look up the typeinfo.  *)
-
-(* Remark. Stack-allocated continuations (and stack-allocated data records)
-   must not "escape upwards", i.e. they must not be stored into data records
-   nor passed to stack-allocated continuation functions.  This discipline is
-   enforced by the tagging system.  The type of a function (or data record)
-   includes its tag.  It must always be possible to partition the tags into
-   two sets, the escaping and the nonescaping, such that nonescaping
-   functions have all nonescaping parameters.  This is a wellformedness
-   property of a tdict:  [tdict_wellformed TD]
- *)
-
-Definition may_escape_type (TD: tdict) (may_escape: tag -> bool) (t: type) : bool :=
-  match TDict.get t TD with
-    | Some (Tdata cl) => existsb (Basics.compose may_escape fst) cl
-    | Some (Tfun c _) => may_escape c
-    | Some (Tother c) => may_escape c
-    | _ => true
+(** retrieve the cTyInfo for a given cTag *)
+Definition get_cTyInfo (c : cTag) : cState cTyInfo :=
+  p <- get ;;
+  let '(n, m, e) := p in
+  match M.get c e with
+    | Some t => ret t
+    | None => ret unkownTyInfo (* Should never get here *)
   end.
 
-Definition tdict_type_ok (TD: tdict) (may_escape: tag -> bool) : Prop :=
-  forall t,
-    match t with             
-      | Some (Tfun c tl) => 
-        may_escape c = false ->
-        existsb (may_escape_type TD may_escape) tl = false
-      | _ => True
-    end.
-
-Definition tdict_wellformed (TD: tdict) : Type := sig (tdict_type_ok TD).
-
-Definition tag_primcall : tag := 1%positive. (* tag for calling primitive functions *)
-Definition tag_primreturn : tag := 2%positive. (* tag for "returning" from 
-    primitive functions.  Primitive functions are all inlined, so they don't
-    actually return, but the type system needs this place-holder tag. *)
-
-Inductive subtype (TD: tdict): type -> type -> Prop :=
-| subtype_refl: forall i, 
-                  subtype TD i i
-| subtype_i: forall (i j: type) (t u: typeinfo),
-               TDict.get i TD = Some t ->
-               TDict.get j TD = Some u ->
-               subtypeinfo TD t u ->
-               subtype TD i j
-with subtypeinfo (TD: tdict): typeinfo -> typeinfo -> Prop :=
-     | subtype_data: forall tl tl',
-                       subtype_clist TD tl tl' ->
-                       subtypeinfo TD (Tdata tl) (Tdata tl')
-     | subtype_fun: forall c tl tl',
-                      subtype_list TD tl' tl ->
-                      subtypeinfo TD (Tfun c tl) (Tfun c tl')
-     | subtype_irefl: forall t,
-                        subtypeinfo TD t t
-with subtype_clist  (TD: tdict): list (tag* list type) -> list (tag* list type) -> Prop :=
-     | subtype_here: forall c t tl t' tl',
-                       subtype_list TD t t' ->
-                       subtype_clist TD tl tl' ->
-                       subtype_clist TD ((c,t)::tl) ((c,t')::tl')
-     | subtype_skip: forall c t tl tl',
-                       subtype_clist TD tl tl' ->
-                       subtype_clist TD tl ((c,t)::tl')
-     | subtype_cnil: subtype_clist TD nil nil
-with subtype_list (TD: tdict): list type -> list type -> Prop :=
-     | subtype_cons: forall t tl t' tl',
-                       subtype TD t t' ->
-                       subtype_list TD tl tl' ->
-                       subtype_list TD (t::tl) (t'::tl')
-     | subtype_nil: subtype_list TD nil nil.
-
-Definition tenv := M.t type.
-
-Require Import ExtLib.Structures.Monads.
-Require Import ExtLib.Data.Monads.OptionMonad.
-Import MonadNotation.
-Open Scope monad_scope.
-
-(* this might even work, but it's not general enough to be useful:
-
-Definition getSome {A} {B}  (f: A -> option B) (o: option A) :=
-  match o with None => None | Some x => f x end.
-
-Notation "'let' 'Some' x '<-' c1 ;; c2" := 
-     (@pbind option _ _ _ _ c1 (getSome (fun x => c2)))
-    (at level 100, c2 at next level, c1 at next level, right associativity) : monad_scope.
- *)
-
-(* [cl_of_casecont TD Gamma ct] is given a list of tagged continuations,
-     and returns the corresponding list of tagged typelists, by looking 
-     up each continuation (variable) to get the types of its parameters. 
- *)
-Definition cl_of_casecont (TD: tdict) (Gamma: tenv) (ct: tag*var) 
-: option (tag * list type) :=
-  t' <- M.get (snd ct) Gamma ;;
-  f <- TDict.get t' TD ;;
-  match f with
-    | Tfun c2 (t2::nil) =>
-      d <- TDict.get t2 TD ;;
-        match d with
-          | (Tdata ((c,t3)::nil)) => ret (fst ct, t3)
-          | _ => None
-        end
-    | _ => None end.
-
-Fixpoint fundefs_lists (f: fundefs) : (list var * list type * list (list var) * list exp)%type :=
-  match f with
-    | Fcons x t ys e' f' => match fundefs_lists f' with
-                              | (xs, ts, yss, es) => (x::xs, t::ts, ys::yss, e'::es)
-                            end
-    | Fnil => (nil,nil,nil,nil)
-  end.
-
-Inductive welltyped (TD: tdict): forall (Gamma: tenv) (e: exp), Prop :=
-| WTconstr: forall tll (tl ytl: list type) (Gamma: tenv) x t c ys e,
-              TDict.get t TD = Some (Tdata tll) ->
-              findtag tll c = Some tl ->
-              getlist ys Gamma = Some ytl ->
-              subtype_list TD ytl tl ->
-              welltyped TD (M.set x t Gamma) e ->
-              welltyped TD Gamma (Econstr x t c ys e)
-| WTcase: forall Gamma y t (tl : list (tag * list type))  cl,
-            M.get y Gamma = Some t ->
-            TDict.get t TD = Some (Tdata tl) ->
-            Forall (fun te => welltyped TD Gamma (snd te)) cl ->
-            welltyped TD Gamma (Ecase y cl)
-| WTproj: forall ty c tl t' Gamma x t n y e,
-            M.get y Gamma = Some ty ->
-            TDict.get ty TD = Some (Tdata ((c,tl)::nil)) ->
-            nthN tl n = Some t' ->
-            subtype TD t' t ->
-            welltyped TD (M.set x t Gamma) e ->
-            welltyped TD Gamma (Eproj x t n y e)
-| WTfun: forall (Gamma Gamma': tenv) fl e,
-           match fundefs_lists fl with (xs,ts,yss,es) => setlist xs ts Gamma = Some Gamma' end ->
-           welltyped_funbodies TD Gamma' fl ->
-           welltyped TD Gamma' e ->
-           welltyped TD Gamma (Efun fl e)
-| WTapp: forall Gamma t c tl ytl f ys,
-           M.get f Gamma = Some t ->
-           TDict.get t TD = Some (Tfun c tl) ->
-           getlist ys Gamma = Some ytl ->
-           subtype_list TD ytl tl ->
-           welltyped TD Gamma (Eapp f ys)
-| WTprim: forall tf ts tk ts' t' Gamma x t f ys e,
-            getlist (f::ys) Gamma = Some (tf::ts) ->
-            TDict.get tf TD = Some (Tfun tag_primcall (tk::ts')) ->
-            TDict.get tk TD = Some (Tfun tag_primreturn (t'::nil)) ->
-            subtype_list TD ts ts' ->
-            subtype TD t' t ->
-            welltyped TD (M.set x t Gamma) e ->
-            welltyped TD Gamma (Eprim x t f ys e)                   
-with welltyped_funbodies (TD: tdict): forall (Gamma: tenv) (fbody: fundefs), Prop :=
-     | WTbody: forall tl Gamma Gamma' f c t ys e fbody',
-                 TDict.get t TD = Some (Tfun c tl) ->
-                 setlist ys tl Gamma = Some Gamma'  ->
-                 welltyped TD Gamma' e ->
-                 welltyped_funbodies TD Gamma (Fcons f t ys e fbody')
-     | WTnil: forall Gamma, welltyped_funbodies TD Gamma Fnil.
+(** add a record type of a given arity to the state and get back relevant tag info
+    (helpful for closure conversion) *)
+Definition makeRecord (n : nat) : cState (cTag * iTag) :=
+  ct <- get_cTag ;;
+  it <- get_iTag ;;
+  _ <- set_cTyInfo ct (it, N.of_nat n, 0%N) ;;
+  ret (ct , it).
