theories/L6_PCPS/ctx_approx.v
@@ -11,14 +11,15 @@ Ltac inv H := inversion H; clear H; subst.
 Section ctx_approx.
 
   Variable pr : prims.
+  Variable cenv : cEnv.
 
   Open Scope ctx_scope.
   
   (** Contextual approximation *)
   Definition ctx_approx : relation exp :=
     fun e1 e2 =>
-      forall C i v1, bstep_e pr empty_env (C |[ e1 ]|) v1 i ->
-                exists v2 j, bstep_e pr empty_env (C |[ e2 ]|) v2 j.
+      forall C i v1, bstep_e pr cenv empty_env (C |[ e1 ]|) v1 i ->
+                exists v2 j, bstep_e pr cenv empty_env (C |[ e2 ]|) v2 j.
   
   (** Contextual equivalence *)
   Definition ctx_equiv : relation exp :=
@@ -48,34 +49,33 @@ Section ctx_approx.
   Qed.
 
   Lemma preord_exp_sound e1 e2 :
-    (forall k rho1 rho2, preord_env_P pr (occurs_free e1) k rho1 rho2 ->
-                    preord_exp pr k (e1, rho1) (e2, rho2)) ->
+    (forall k rho1 rho2, preord_env_P pr cenv (occurs_free e1) k rho1 rho2 ->
+                    preord_exp pr cenv k (e1, rho1) (e2, rho2)) ->
     ctx_approx e1 e2.
   Proof.
     intros Hyp C i v1 Hstep.
     assert (Hyp' := Hyp).
-    eapply (preord_exp_compat pr i empty_env empty_env C) in Hyp;
+    eapply (preord_exp_compat pr cenv i empty_env empty_env C) in Hyp;
       [| now eapply preord_env_P_refl ].
     edestruct Hyp as [v2 [c2 [Hstep2 Hpre2]]]; eauto.
   Qed.
   
   Definition x : var := 1%positive.
   Definition y : var := 2%positive.
-  
-  Definition tau : type := 1%positive.
-  Definition c : tag := 1%positive.
-  
+  Definition c : cTag := 1%positive.
+  Definition f : fTag := 1%positive.
+
   Definition stuck : exp :=
-    Econstr x tau c [] (
-              Econstr y tau c [] (
-                        Eapp x [y])).
+    Econstr x  c [] (
+              Econstr y c [] (
+                        Eapp x f [y])).
   
   Lemma stuck_gets_stuck rho :
-    ~ (exists v c, bstep_e pr rho stuck v c).
+    ~ (exists v c, bstep_e pr cenv rho stuck v c).
   Proof.
-    intros [v [c H]]. inv H. inv H8.
-    inv H10. inv H7. inv H9.
-    rewrite M.gso, M.gss in H1. inv H1.
+    intros [v [c H]]. inv H. inv H7.
+    inv H9. inv H6. inv H8.
+    rewrite M.gso, M.gss in H2. inv H2.
     intros Hc. inv Hc.
   Qed.
   
