theories/L6_PCPS/logical_relations.v
@@ -1,13 +1,17 @@
 Require Import Coq.NArith.BinNat Coq.Relations.Relations Coq.MSets.MSets Coq.MSets.MSetRBT
         Coq.Lists.List Coq.omega.Omega Coq.Sets.Ensembles.
-Require Import cps eval cps_util identifiers env ctx Ensembles_util List_util.
+Require Import cps eval cps_util identifiers ctx Ensembles_util List_util.
 Import ListNotations.
 
 
 Section Log_rel.
 
   Variable (pr : prims).
-
+  Variable (cenv : cEnv).
+  
+  (* Tag for closure records *)
+  Variable (clo_tag : cTag). 
+  
   (** step-indexed preorder on cps terms *)
   (* Expression relation : 
    * ---------------------
@@ -30,8 +34,8 @@ Section Log_rel.
         let '(e1, rho1) := p1 in
         let '(e2, rho2) := p2 in
         forall v1 c1,
-           c1 <= k -> bstep_e pr rho1 e1 v1 c1 ->
-           exists v2 c2, bstep_e pr rho2 e2 v2 c2 /\ 
+           c1 <= k -> bstep_e pr cenv rho1 e1 v1 c1 ->
+           exists v2 c2, bstep_e pr cenv rho2 e2 v2 c2 /\ 
                     preord_val (k - c1) v1 v2
     in
     let fix preord_val_aux (v1 v2 : val) {struct v1} : Prop :=
@@ -45,13 +49,13 @@ Section Log_rel.
         in
         match v1, v2 with
           | Vfun rho1 defs1 f1, Vfun rho2 defs2 f2 =>
-            forall (vs1 vs2 : list val) (j : nat) (t1 : type) 
+            forall (vs1 vs2 : list val) (j : nat) (t : fTag) 
               (xs1 : list var) (e1 : exp) (rho1' : env),
               length vs1 = length vs2 ->
-              find_def f1 defs1 = Some (t1, xs1, e1) ->
+              find_def f1 defs1 = Some (t, xs1, e1) ->
               Some rho1' = setlist xs1 vs1 (def_funs defs1 defs1 rho1 rho1) ->
-              exists (t2 : type) (xs2 : list var) (e2 : exp) (rho2' : env),
-                find_def f2 defs2 = Some (t2, xs2, e2) /\
+              exists (xs2 : list var) (e2 : exp) (rho2' : env),
+                find_def f2 defs2 = Some (t, xs2, e2) /\
                 Some rho2' = setlist xs2 vs2 (def_funs defs2 defs2 rho2 rho2) /\
                 match k with
                   | 0 => True
@@ -61,7 +65,7 @@ Section Log_rel.
                     Forall2 R vs1 vs2 ->
                     preord_exp (k - (k-j)) (e1, rho1') (e2, rho2')
                 end
-          | Vconstr tau1 t1 vs1, Vconstr tau2 t2 vs2 =>
+          | Vconstr t1 vs1, Vconstr t2 vs2 =>
             t1 = t2 /\ Forall2_aux vs1 vs2
           | Vint n1, Vint n2 => n1 = n2
           | _, _ => False
@@ -72,25 +76,25 @@ Section Log_rel.
     let '(e1, rho1) := p1 in
     let '(e2, rho2) := p2 in
     forall v1 c1,
-      c1 <= k -> bstep_e pr rho1 e1 v1 c1 ->
-      exists v2 c2, bstep_e pr rho2 e2 v2 c2 /\
+      c1 <= k -> bstep_e pr cenv rho1 e1 v1 c1 ->
+      exists v2 c2, bstep_e pr cenv rho2 e2 v2 c2 /\
                preord_val (k - c1) v1 v2.
-
+  
   (** more compact definition of the value preorder *)
   Definition preord_val' (k : nat) (v1 v2 : val) : Prop :=
     match v1, v2 with
       | Vfun rho1 defs1 f1, Vfun rho2 defs2 f2 =>
-        forall (vs1 vs2 : list val) j (t1 : type) (xs1 : list var)
+        forall (vs1 vs2 : list val) j (t : fTag) (xs1 : list var)
                (e1 : exp) (rho1' : env),
           length vs1 = length vs2 -> 
-          find_def f1 defs1 = Some (t1, xs1, e1) ->
+          find_def f1 defs1 = Some (t, xs1, e1) ->
           Some rho1' = setlist xs1 vs1 (def_funs defs1 defs1 rho1 rho1) ->
-          exists (t2 : type) (xs2 : list var) (e2 : exp) (rho2' : env),
-            find_def f2 defs2 = Some (t2, xs2, e2) /\
+          exists (xs2 : list var) (e2 : exp) (rho2' : env),
+            find_def f2 defs2 = Some (t, xs2, e2) /\
             Some rho2' = setlist xs2 vs2 (def_funs defs2 defs2 rho2 rho2) /\
             (j < k -> Forall2 (preord_val j) vs1 vs2 ->
              preord_exp j (e1, rho1') (e2, rho2'))
-      | Vconstr tau1 t1 vs1, Vconstr tau2 t2 vs2 =>
+      | Vconstr t1 vs1, Vconstr t2 vs2 =>
         t1 = t2 /\ Forall2_asym (preord_val k) vs1 vs2
       | Vint n1, Vint n2 => n1 = n2
       | _, _ => False
@@ -114,7 +118,7 @@ Section Log_rel.
         intros H; split; inv H; eauto. inv H1.
         split; [ now eauto | now eapply IHxs ].
     - split; intros Hpre; simpl; intros; 
-      edestruct (Hpre vs1 vs2 0) as [t2 [xs2 [e2 [rho' [H1' [H2' H3']]]]]];
+      edestruct (Hpre vs1 vs2 0) as [xs2 [e2 [rho' [H1' [H2' H3']]]]];
       eauto; do 4 eexists; repeat split; eauto; intros Hc; exfalso; omega.
     - revert l0; induction l as [| x xs IHxs];
       intros l2; destruct l2 as [| y ys ];
@@ -125,8 +129,8 @@ Section Log_rel.
       + inv H. inv H1. split. reflexivity.
         split. now eauto. eapply IHxs. split; eauto. 
     - split; intros Hpre; simpl; intros; 
-      now (edestruct Hpre as [t2 [xs2 [e2 [rho' [H1' [H2' H3']]]]]]; eauto;
-           do 4 eexists; do 2 (split; eauto); intros Hleq Hf v1 c1 Hleq' Hstep;
+      now (edestruct Hpre as [xs2 [e2 [rho' [H1' [H2' H3']]]]]; eauto;
+           do 3 eexists; do 2 (split; eauto); intros Hleq Hf v1 c1 Hleq' Hstep;
            (assert (Heq : k - (k - j) = j) by omega); rewrite Heq in *;
            eapply H3'; eauto).
   Qed.
@@ -370,11 +374,11 @@ Section Log_rel.
     - inv Hpre. inv H0.
       split; auto. constructor; eauto; rewrite preord_val_eq in *.
       eapply IHv1; eauto.
-      destruct (IHv0 ((Vconstr tau t1 l'))) as [Heq Hpre']; eauto.
+      destruct (IHv0 ((Vconstr c l'))) as [Heq Hpre']; eauto.
       simpl. split; eauto.
     - intros vs1 vs2 j t1 xs e1 rho1' Hlen Hf Heq.
-      edestruct Hpre as [t2 [xs2 [e2 [rho2' [H1 [H2 H3]]]]]]; eauto.
-      do 4 eexists; split; eauto. split; eauto. intros Hleq' Hall. 
+      edestruct Hpre as [xs2 [e2 [rho2' [H1 [H2 H3]]]]]; eauto.
+      do 3 eexists; split; eauto. split; eauto. intros Hleq' Hall. 
       eapply H3; eauto. omega. 
   Qed.
   
@@ -408,13 +412,13 @@ Section Log_rel.
   
   (** * Compatibility Properties *)
 
-  Lemma preord_exp_const_compat k rho1 rho2 x x' tau t ys1 ys2 e1 e2 :
+  Lemma preord_exp_const_compat k rho1 rho2 x x' t ys1 ys2 e1 e2 :
     Forall2 (preord_var_env k rho1 rho2) ys1 ys2 ->
     (forall vs1 vs2 : list val,
        Forall2 (preord_val k) vs1 vs2 ->
-       preord_exp k (e1, M.set x (Vconstr tau t vs1) rho1)
-                  (e2, M.set x' (Vconstr tau t vs2) rho2)) ->
-    preord_exp k (Econstr x tau t ys1 e1, rho1) (Econstr x' tau t ys2 e2, rho2).
+       preord_exp k (e1, M.set x (Vconstr t vs1) rho1)
+                  (e2, M.set x' (Vconstr t vs2) rho2)) ->
+    preord_exp k (Econstr x t ys1 e1, rho1) (Econstr x' t ys2 e2, rho2).
   Proof.
     intros Hall Hpre v1 c1 Hleq1 Hstep1. inv Hstep1.
     edestruct (preord_var_env_getlist rho1 rho2) as [vs2' [Hget' Hpre']];
@@ -447,17 +451,17 @@ Section Log_rel.
     intros H. induction H; eauto.
   Qed.    
   
-  Lemma preord_exp_app_compat k rho1 rho2 x1 x2 ys1 ys2 :
+  Lemma preord_exp_app_compat k rho1 rho2 x1 x2 ft ys1 ys2 :
     preord_var_env k rho1 rho2 x1 x2 ->
     Forall2 (preord_var_env k rho1 rho2) ys1 ys2 ->
-    preord_exp k (Eapp x1 ys1, rho1) (Eapp x2 ys2, rho2).
+    preord_exp k (Eapp x1 ft ys1, rho1) (Eapp x2 ft ys2, rho2).
   Proof.
     intros Hvar Hall v1 c1 Hleq1 Hstep1. inv Hstep1.
     edestruct Hvar as [v2' [Hget Hpre]]; eauto.
     rewrite preord_val_eq in Hpre.
     destruct v2'; try (now simpl in Hpre; contradiction).
     edestruct preord_var_env_getlist as [vs2 [Hget' Hpre']]; eauto.
-    edestruct (Hpre vs vs2 (k-1)) as [t2 [xs2 [e2 [rho2' [Hf [Hset H']]]]]]; eauto.
+    edestruct (Hpre vs vs2 (k-1)) as [xs2 [e2 [rho2' [Hf [Hset H']]]]]; eauto.
     now eapply Forall2_length; eauto.
     edestruct H' with (c1 := c) as [v2 [c2 [Hstep' Hpre'']]];
       eauto; try omega.
@@ -470,10 +474,11 @@ Section Log_rel.
   Lemma preord_exp_case_nil_compat k rho1 rho2 x1 x2 :
     preord_exp k (Ecase x1 [], rho1) (Ecase x2 [], rho2).
   Proof.
-    intros v1 c1 Hleq1 Hstep1. inv Hstep1. inv H3.
+    intros v1 c1 Hleq1 Hstep1. inv Hstep1. inv H4.
   Qed.
-
+  
   Lemma preord_exp_case_cons_compat k rho1 rho2 x1 x2 c e1 e2 P1 P2:
+    Forall2 (fun p p' => fst p = fst p') P1 P2 ->
     preord_var_env k rho1 rho2 x1 x2 ->
     preord_exp k (e1, rho1) (e2, rho2) ->
     preord_exp k (Ecase x1 P1, rho1)
@@ -481,20 +486,23 @@ Section Log_rel.
     preord_exp k (Ecase x1 ((c, e1) :: P1), rho1)
                (Ecase x2 ((c, e2) :: P2), rho2).
   Proof.
-    intros Henv Hexp_hd Hexp_tl v1 c1 Hleq1 Hstep1. inv Hstep1. inv H3.
+    intros Hall Henv Hexp_hd Hexp_tl v1 c1 Hleq1 Hstep1. inv Hstep1. inv H4.
     destruct (M.elt_eq c t) eqn:Heq; subst.
     - inv H0. edestruct Hexp_hd as [v2 [c2 [Hstep2 Hpre2]]]; eauto.
       edestruct Henv as [v2' [Hget Hpre]]; eauto.
       rewrite preord_val_eq in Hpre.
       destruct v2'; try (now simpl in Hpre; contradiction). inv Hpre. 
-      repeat eexists; eauto. econstructor; eauto. simpl; rewrite Heq; eauto.
-    - edestruct Hexp_tl as [v2 [c2 [Hstep2 Hpre2]]]; eauto.
+      repeat eexists; eauto. econstructor; eauto; [| now simpl; rewrite Heq; eauto ].
+      inv H2. econstructor; try now eauto.
+      eapply caseConsistent_same_cTags; eassumption.
+    - edestruct Hexp_tl as [v2 [c2 [Hstep2 Hpre2]]]; eauto. inv H2.
       econstructor; eauto. inv Hstep2.
       edestruct Henv as [v2' [Hget Hpre]]; eauto.
       rewrite preord_val_eq in Hpre.
       destruct v2'; try (now simpl in Hpre; contradiction). inv Hpre.
-      rewrite Hget in H3; inv H3.
-      repeat eexists; eauto. econstructor; eauto. simpl; rewrite Heq; eauto.
+      rewrite Hget in H4; inv H4.
+      repeat eexists; eauto. econstructor; eauto; [| now simpl; rewrite Heq; eauto ].
+      inv H2. econstructor; try now eauto.
   Qed.
   
   Axiom Prim_axiom :
@@ -507,13 +515,13 @@ Section Log_rel.
           f' vs2 = Some v2 /\                      
           preord_val k v1 v2.
   
-  Lemma preord_exp_prim_compat k rho1 rho2 x1 x2 tau f ys1 ys2 e1 e2 :
+  Lemma preord_exp_prim_compat k rho1 rho2 x1 x2 f ys1 ys2 e1 e2 :
     Forall2 (preord_var_env k rho1 rho2) ys1 ys2 ->
     (forall v1 v2,
        preord_val k v1 v2 -> 
        preord_exp k (e1, M.set x1 v1 rho1)
                   (e2, M.set x2 v2 rho2)) ->
-    preord_exp k (Eprim x1 tau f ys1 e1, rho1) (Eprim x2 tau f ys2 e2, rho2).
+    preord_exp k (Eprim x1 f ys1 e1, rho1) (Eprim x2 f ys2 e2, rho2).
   Proof.
     intros Henv Hexp v1 c1 Hleq1 Hstep1. inv Hstep1.
     edestruct preord_var_env_getlist as [vs2 [Hget' Hpre']]; eauto.
@@ -559,7 +567,7 @@ Section Log_rel.
       + rewrite preord_val_eq.
         intros vs1 vs2 j t1 xs1 e1 rho1' Hlen Hf Hs.
         edestruct setlist_length as [rho2' Hs']; eauto.
-        exists t1. exists xs1. exists e1. exists rho2'. split; eauto.
+        exists xs1. exists e1. exists rho2'. split; eauto.
         split; [ now eauto |]. intros Hleq Hpre'. 
         eapply Hyp. omega.
         eapply preord_env_P_setlist_l; [| | eauto | eauto | eauto]. 
@@ -592,8 +600,9 @@ Section Log_rel.
         rewrite preord_val_eq. constructor; eauto using Forall2_Forall2_asym_included.
     - eapply preord_exp_case_nil_compat.
     - eapply preord_exp_case_cons_compat; eauto.
-      apply IHe. intros x P. apply Henv. constructor; eauto.
-      apply IHe0. intros x P. apply Henv. apply Free_Ecase3; eauto.
+      now apply Forall2_refl.
+      apply IHe. intros x P. apply Henv. now constructor; eauto.
+      apply IHe0. intros x P. apply Henv. now apply Free_Ecase3; eauto.
     - eapply preord_exp_proj_compat; eauto.
       intros v1 v2 Hval. eapply IHe. eapply preord_env_P_extend; eauto.
       eapply preord_env_P_antimon; eauto.
@@ -632,7 +641,7 @@ Section Log_rel.
       + rewrite preord_val_eq.
         intros vs1 vs2 j t1 xs1 e1 rho1' Hlen Hf Hs.
         edestruct setlist_length as [rho2' Hs']; eauto.
-        exists t1. exists xs1. exists e1. exists rho2'. split; eauto.
+        exists xs1. exists e1. exists rho2'. split; eauto.
         split. eauto. intros Hleq Hpre'.
         eapply preord_exp_refl. 
         eapply preord_env_P_setlist_l; [| | eauto | eauto | eauto].
@@ -640,7 +649,8 @@ Section Log_rel.
         eapply (preord_env_P_monotonic _ k); eauto. omega.
         intros x Hin Hfr. 
         apply find_def_correct in Hf.
-        edestruct (occurs_free_in_fun _ _ _ _ _ Hf x Hfr); eauto; try contradiction.
+        edestruct (occurs_free_in_fun _ _ _ _ _ Hf x Hfr);
+          eauto; try contradiction.
         inv H; eauto.
     - simpl. intros x HP. inv HP. apply Hpre; eauto. inv H.
       apply Hpre; eauto. inv H0.
@@ -681,14 +691,15 @@ Section Log_rel.
     - intros.
       edestruct (setlist_length (def_funs f0 f0 t t) (def_funs f0 f0 t t))
         as [rho2' Hset']; eauto.
-      do 4 eexists; split; eauto. split; eauto. intros Hc.
+      do 3 eexists; split; eauto. split; eauto. intros Hc.
       exfalso. omega.
     - split; eauto. constructor; eauto. rewrite preord_val_eq; eauto.
         destruct IHx0. eauto.
     - intros.
       edestruct (setlist_length (def_funs f0 f0 t t) (def_funs f0 f0 t t))
         as [rho2' Hset']; eauto.
-      do 4 eexists; eauto. split; eauto. split; eauto.
+      do 3 eexists; eauto. split; eauto.
+      split; eauto.
       intros Hleq Hall v1 c Hleq' Hstep. 
       eapply preord_exp_refl_weak; eauto.
       eapply preord_env_setlist_l; eauto.
@@ -719,32 +730,54 @@ Section Log_rel.
     (* TODO : this lemma could be used to refactor hoisting correctness proof *)
     induction P1' as [| [c' e'] P1' IHP1']; simpl;
     intros Henv Hexp v1 c1 Hleq1 Hstep1.
-    - inv Hstep1. simpl in H3. edestruct Henv as [v2' [Hget Hpre]]; eauto.
+    - inv Hstep1. simpl in H4. edestruct Henv as [v2' [Hget Hpre]]; eauto.
       rewrite preord_val_eq in Hpre.
       destruct v2'; try (now simpl in Hpre; contradiction). inv Hpre.
-      destruct (M.elt_eq c t1) eqn:Heq; subst.
-      + inv H3. edestruct Hexp as [v2 [c2 [Hstep2 Hpre2]]]; eauto.
-        repeat eexists; eauto. econstructor; eauto. simpl; rewrite Heq; eauto.
+      destruct (M.elt_eq c c0) eqn:Heq; subst.
+      + inv H4. edestruct Hexp as [v2 [c2 [Hstep2 Hpre2]]]; eauto.
+        repeat eexists; eauto.
+        econstructor; [ now eauto | | simpl; rewrite Heq; now eauto | eassumption ].
+        inv H2. econstructor; [ now eauto | now eauto | now eauto |].
+        eapply caseConsistent_same_cTags. now apply Forall2_refl.
+        eassumption.
       + edestruct (preord_exp_refl k e) as [v2 [c2 [Hstep2 Hpre2]]]; eauto.
         * eapply preord_env_P_antimon; [ eassumption | ].
           intros x' H'. eapply occurs_free_Ecase_Included; eauto.
           right. eapply findtag_In_patterns; eauto.
-        * repeat eexists; eauto. econstructor; eauto. simpl; rewrite Heq; eauto.
-    - inv Hstep1. simpl in H3. edestruct Henv as [v2' [Hget Hpre]]; eauto.
+        * repeat eexists; eauto.
+          econstructor; [ now eauto | | simpl; rewrite Heq; now eauto | eassumption ].
+          inv H2. econstructor; [ now eauto | now eauto | now eauto |].
+          eapply caseConsistent_same_cTags. now apply Forall2_refl.
+          eassumption.
+    - inv Hstep1. simpl in H4. edestruct Henv as [v2' [Hget Hpre]]; eauto.
       rewrite preord_val_eq in Hpre.
       destruct v2'; try (now simpl in Hpre; contradiction). inv Hpre.
-      destruct (M.elt_eq c' t1) eqn:Heq; subst.
-      + inv H3.
+      destruct (M.elt_eq c' c0) eqn:Heq; subst.
+      + inv H4.
         edestruct (preord_exp_refl k e) as [v2 [c2 [Hstep2 Hpre2]]]; eauto.
         *eapply preord_env_P_antimon; [ eassumption | ].
           intros x' H'. eapply occurs_free_Ecase_Included; eauto. now left. 
-        * repeat eexists; eauto. econstructor; eauto. simpl; rewrite Heq; eauto.
+        * repeat eexists; eauto.
+          econstructor; [ now eauto | | simpl; rewrite Heq; now eauto | eassumption ].
+          inv H2. econstructor; [ now eauto | now eauto | now eauto |].
+          eapply caseConsistent_same_cTags; [| eassumption ].
+          apply Forall2_app. now apply Forall2_refl.
+          constructor. reflexivity. now apply Forall2_refl.
       + edestruct IHP1' as [v2 [c2 [Hstep2 Hpre2]]]; eauto; eauto.
         * eapply preord_env_P_antimon; [ eassumption | ].
           intros x' H'. eapply Free_Ecase3; eauto. 
         * econstructor; eauto.
-        * inv Hstep2. rewrite Hget in H4; inv H4.
-          repeat eexists; eauto. econstructor; eauto. simpl. rewrite Heq; eauto.
+          inv H2.
+          eapply caseConsistent_same_cTags; [| eassumption ].
+          apply Forall2_app. now apply Forall2_refl.
+          constructor. reflexivity. now apply Forall2_refl.
+        * inv Hstep2. rewrite Hget in H5; inv H5.
+          repeat eexists; eauto.
+          econstructor; [ now eauto | | simpl; rewrite Heq; now eauto | eassumption ].
+          inv H2. econstructor; [ now eauto | now eauto | now eauto |].
+          eapply caseConsistent_same_cTags; [| eassumption ].
+          apply Forall2_app. now apply Forall2_refl.
+          constructor. reflexivity. now apply Forall2_refl.
   Qed.
 
   (* TODO : move *)
@@ -789,10 +822,10 @@ Section Log_rel.
       intros vs1 vs2 j t1 xs1 e' rho1' Hlen Hf Hs.
       edestruct find_def_def_funs_ctx as [H1 | [c [H1 H2]]]; eauto.
       + edestruct setlist_length as [rho2' Hs']; eauto.
-        do 5 eexists; eauto. split; eauto.
+        do 4 eexists; eauto. split; eauto.
         intros Hleq Hall.
         eapply preord_exp_refl.
-        eapply preord_env_P_setlist_l; [| | eauto | eauto | eauto ].
+        eapply preord_env_P_setlist_l; [| | now eauto | now eauto | now eauto ].
         eapply IH'; eauto. 
         intros. eapply Hpre; eauto. omega. 
         eapply preord_env_P_monotonic; [| eassumption ]. omega.
@@ -801,7 +834,7 @@ Section Log_rel.
         eapply occurs_free_in_fun in Hfv; eauto.
         inv Hfv. exfalso. eauto. right. eapply Union_sym. eauto.
       + subst. edestruct setlist_length as [rho2' Hs']; eauto.
-        do 5 eexists; eauto. split; eauto.
+        do 4 eexists; eauto. split; eauto.
         intros Hleq Hall. eapply Hpre; eauto.
         eapply preord_env_P_setlist_l; [| | eauto | eauto | eauto ].
         eapply IH'; eauto.
@@ -905,7 +938,7 @@ Section Log_rel.
   (** Expression relation is transitive *)
   Lemma preord_exp_trans_pre (k : nat) :
     (* The induction hypothesis for transitivity of
-       the value relation. They need to be proved simultaneously *)
+       the value relation. *)
     (forall k' v1 v2 v3,
        k' <= k ->
        preord_val k' v1 v2 ->
@@ -948,8 +981,8 @@ Section Log_rel.
         inv H2. now inv H1.
       + assert
           (Hsuf :
-             preord_val k (Vconstr tau t3 l) (Vconstr tau t3 l')).
-        { eapply IHx0 with (v2 := Vconstr tau t3 l0); [| intros m];
+             preord_val k (Vconstr c0 l) (Vconstr c0 l')).
+        { eapply IHx0 with (v2 := Vconstr c0 l0); [| intros m];
           rewrite !preord_val_eq in *. simpl. split; eauto.
           specialize (H2 m). rewrite !preord_val_eq in H2.
           split; eauto. inv H2. now inv H1. }
@@ -957,14 +990,14 @@ Section Log_rel.
     - intros H1 H2. assert (H2' := H2 k); rewrite !preord_val_eq in *.
       destruct v1; destruct v2; try (now simpl in *; contradiction).
       intros vs1 vs3 j t1' xs1 e1 rho1' Hlen Hf Hs.
-      edestruct (H1 vs1 vs3) as [t2' [xs2 [e2 [rho2 [Hf2 [Hs2 Hpre2]]]]]]; eauto.
-      edestruct (H2' vs3 vs3) with (j := 0) as [t3' [xs3 [e3 [rho3 [Hf3 [Hs3 Hpre3]]]]]]; eauto.
-      do 4 eexists; split; eauto. split; eauto. intros Hlt Hall.
+      edestruct (H1 vs1 vs3) as [xs2 [e2 [rho2 [Hf2 [Hs2 Hpre2]]]]]; eauto.
+      edestruct (H2' vs3 vs3) with (j := 0) as [xs3 [e3 [rho3 [Hf3 [Hs3 Hpre3]]]]]; eauto.
+      do 3 eexists; split; eauto. split; eauto. intros Hlt Hall.
       eapply preord_exp_trans_pre. intros. eapply H; eauto. omega.
       eapply Hpre2; eauto.
       intros m. specialize (H2 (m + 1)). rewrite !preord_val_eq in H2.
       edestruct (H2 vs3 vs3) with (j := m)
-        as [t3'' [xs3' [e3' [rho3' [Hf3' [Hs3' Hpre3']]]]]]; eauto.
+        as [xs3' [e3' [rho3' [Hf3' [Hs3' Hpre3']]]]]; eauto.
       rewrite Hf3 in Hf3'. inv Hf3'. rewrite <- Hs3 in Hs3'. inv Hs3'.
       eapply Hpre3'; eauto. omega. eapply Forall2_refl. now eapply preord_val_refl.
   Qed.
@@ -1010,7 +1043,7 @@ Section Log_rel.
       + rewrite preord_val_eq.
         intros vs1 vs2 j t1 xs1 e1 rho1' Hlen Hf Hs.
         edestruct setlist_length as [rho2' Hs']; eauto.
-        exists t1. exists xs1. exists e1. exists rho2'. split; eauto.
+        exists xs1. exists e1. exists rho2'. split; eauto.
         split. eauto. intros Hleq Hpre. 
         eapply Hyp2; try omega.
         eapply preord_env_P_setlist_l; eauto.
@@ -1020,8 +1053,8 @@ Section Log_rel.
     - simpl. eauto.
   Qed.
 
-  (* TODO fix typo *)
-  Lemma preord_exp_proord_env_com rho1 rho2 rho1' rho2' e1 e2 :
+  (** Commutativity property *)  
+  Lemma preord_exp_preord_env_com rho1 rho2 rho1' rho2' e1 e2 :
     (forall k, preord_exp k (e1, rho1) (e2, rho2)) ->
     (forall k, preord_env_P (occurs_free e1) k rho1' rho1) ->
     (forall k, preord_env_P (occurs_free e2) k rho2 rho2') ->
@@ -1238,7 +1271,7 @@ Section Log_rel.
       + rewrite preord_val_eq.
         intros vs1 vs2 j t1 xs1 e1 rho1' Hlen Hf Hs.
         edestruct setlist_length as [rho2' Hs']; eauto.
-        exists t1. exists xs1. exists e1. exists rho2'. split; eauto.
+        exists xs1. exists e1. exists rho2'. split; eauto.
         specialize (find_def_name_in_fundefs _ _ _ Hf); intros Hname.
         destruct (@Dec _ _  (Decidable_name_in_fundefs B2) v).
         exfalso. inv HD2. eapply H0; eauto.
@@ -1276,7 +1309,7 @@ Section Log_rel.
     intros f tau xs e B1 B2 rho1 rho2 Hcl1 Hcl2 Hun HD Hyp. rewrite preord_val_eq.
     intros vs1 vs2 j t1 xs1 e1 rho1' Hlen Hf Hs.
     edestruct setlist_length as [rho2' Hs']; eauto. simpl in Hf.
-    destruct (M.elt_eq f f); try congruence. inv Hf. do 4 eexists. split. simpl.
+    destruct (M.elt_eq f f); try congruence. inv Hf. do 3 eexists. split. simpl.
     destruct (M.elt_eq f f); try congruence. eauto. split; eauto.
     intros Hleq Hpre'. simpl in Hs, Hs'. rewrite def_funs_append in Hs'.
     intros v1 c1 Hleq1 Hstep1. inv Hstep1. edestruct preord_exp_refl; eauto.
@@ -1364,7 +1397,7 @@ Section Log_rel.
         * eapply preord_val_def_funs_append_pre; eauto.
         * rewrite preord_val_eq. intros vs1 vs2 j t1 xs1 e1 rho1'' Hlen Hf Hs.
           edestruct setlist_length as [rho2'' Hs']; [eauto | | ]. eauto.
-          exists t1, xs1, e1, rho2''. repeat split; eauto.
+          exists xs1, e1, rho2''. repeat split; eauto.
           simpl in *. destruct (M.elt_eq v f); try congruence.
           specialize (find_def_name_in_fundefs _ _ _ Hf); intros Hname.
           erewrite <- find_def_fundefs_append_l in Hf; eauto.
@@ -1466,7 +1499,7 @@ Section Log_rel.
           rewrite Setminus_Empty_set. apply preord_env_Empty_set.
           { rewrite preord_val_eq. intros vs1 vs2 j t1 xs1 e1 rho1'' Hlen Hf Hs.
             edestruct setlist_length as [rho2'' Hs']; [eauto | | ]. eauto.
-            exists t1, xs1, e1, rho2''. repeat split; eauto.
+            exists xs1, e1, rho2''. repeat split; eauto.
             erewrite <- find_def_split_fds; eauto.
             intros Hleq Hpre'. eapply preord_exp_refl; eauto.
             eapply preord_env_P_setlist_l; [| | | eauto | eauto ]; eauto. }
@@ -1508,7 +1541,7 @@ Section Log_rel.
           rewrite Setminus_Empty_set. apply preord_env_Empty_set.
           { rewrite preord_val_eq. intros vs1 vs2 j t1 xs1 e1 rho1'' Hlen Hf Hs.
             edestruct setlist_length as [rho2'' Hs']; [eauto | | ]. eauto.
-            exists t1, xs1, e1, rho2''. repeat split; eauto.
+            exists xs1, e1, rho2''. repeat split; eauto.
             erewrite <- find_def_split_fds; eauto.
             intros Hleq Hpre'. eapply preord_exp_refl; eauto.
             eapply preord_env_P_setlist_l; [| | | eauto | eauto ]; eauto. }
@@ -1562,7 +1595,7 @@ Section Log_rel.
         eapply preord_env_P_antimon; [ eapply IHB1; eauto |].
         rewrite (fundefs_append_fun_in_fundefs B B' (fundefs_append B B')); eauto.
         rewrite HS. simpl in HS1.
-        rewrite <- (Setminus_Disjoint (fun_in_fundefs B1) (Singleton _ (v, t, l, e))).
+        rewrite <- (Setminus_Disjoint (fun_in_fundefs B1) (Singleton _ (v, f, l, e))).
         rewrite <- Setminus_Union_Inlcluded; eauto using Included_refl.
         eapply Included_Setminus_compat; eauto using Included_refl.
         now rewrite Union_sym.  
@@ -1578,7 +1611,7 @@ Section Log_rel.
           rewrite Setminus_Empty_set. apply preord_env_Empty_set.
           rewrite preord_val_eq. intros vs1 vs2 j t1 xs1 e1 rho1'' Hlen Hf Hs. 
           edestruct setlist_length as [rho2'' Hs']; [eauto | | ]. eauto.
-          exists t1, xs1, e1, rho2''. repeat split; eauto.
+          exists xs1, e1, rho2''. repeat split; eauto.
           erewrite <- find_def_Included_fun_in_fundefs; eauto.
           eapply fun_in_fundefs_name_in_fundefs. now eapply find_def_correct; eauto.
           intros Hleq Hpre'. eapply preord_exp_refl; eauto. 
@@ -1683,7 +1716,7 @@ Section Log_rel.
           rewrite Setminus_Empty_set. apply preord_env_Empty_set.
           rewrite preord_val_eq. intros vs1 vs2 j t1 xs1 e1 rho1'' Hlen Hf Hs. 
           edestruct setlist_length as [rho2'' Hs']; [eauto | | ]. eauto.
-          exists t1, xs1, e1, rho2''. repeat split; eauto.
+          exists xs1, e1, rho2''. repeat split; eauto.
           erewrite <- find_def_Same_set_fun_in_fundefs; eauto.
           intros Hleq Hpre'. eapply preord_exp_refl; eauto.
           eapply preord_env_P_setlist_l; [| | | eauto | eauto ]; eauto.
@@ -1693,854 +1726,860 @@ Section Log_rel.
       simpl. eauto.
   Qed.
 
-(** step-indexed relation on cps terms. Relates
- * cps-terms with closure-converted terms  *)
-(* Expression relation : 
- * ---------------------
- *  (e1, ρ1) ~_k (e2, ρ2) iff 
- *    forall c1 <= k, 
- *      ρ1 |- e1 ->^c1 v1 -> 
- *      exists v2, p2 |- e2 -> v2 /\ v1 ~_(k-c1) v2 
- * Value relation :
- * ----------------
- * Integers: (n1 ~_k n2) iff n1 = n2
- * Constructors: C[v_1, .., v_n] ~_k C[v'_1, .., v'_m] iff
+  (** step-indexed relation on cps terms. Relates
+   * cps-terms with closure-converted terms  *)
+  (* Expression relation : 
+   * ---------------------
+   *  (e1, ρ1) ~_k (e2, ρ2) iff 
+   *    forall c1 <= k, 
+   *      ρ1 |- e1 ->^c1 v1 -> 
+   *      exists v2, p2 |- e2 -> v2 /\ v1 ~_(k-c1) v2 
+   * Value relation :
+   * ----------------
+   * Integers: (n1 ~_k n2) iff n1 = n2
+   * Constructors: C[v_1, .., v_n] ~_k C[v'_1, .., v'_m] iff
                      n <= m /\ v_1 ~_k v'_1 /\ ... /\ v_n ~_k v'_n'
  * Closures: (\f1 x1. e1, ρ1) ~_k {(\f2 Γ x2. e2, ρ2); ρ} iff 
  *              \forall v1 v2 i < k, v1 ~_j v2 => 
  *                (e1, ρ1[x1 -> v1, f1 -> (\f1 x1. e1, ρ1)]) ~_j 
  *                (e2, [x2 -> v2, f2 -> (\f2 x2. e2, ρ2), Γ -> ρ])
  *)
-Fixpoint cc_approx_val (k : nat) (v1 v2 : val) {struct k} : Prop :=
-  let cc_approx_exp (k : nat) (p1 p2 : exp * env) : Prop :=
-      let '(e1, rho1) := p1 in
-      let '(e2, rho2) := p2 in
-      forall v1 c1,
-        c1 <= k -> bstep_e pr rho1 e1 v1 c1 ->
-        exists v2 c2, bstep_e pr rho2 e2 v2 c2 /\ 
-                 cc_approx_val (k - c1) v1 v2
-  in
-  let fix cc_approx_val_aux (v1 v2 : val) {struct v1} : Prop :=
-      let fix Forall2_aux vs1 vs2 :=
-          match vs1, vs2 with
-            | [], _ => True
-            | v1 :: vs1, v2 :: vs2 =>
-              cc_approx_val_aux v1 v2 /\ Forall2_aux vs1 vs2
-            | _, _ => False
-          end
-      in
-      match v1, v2 with
-        | Vfun rho1 defs1 f1,
-          Vconstr tau t ((Vfun rho2 defs2 f2) ::  (Vconstr tau' t' fvs) :: l)  =>
-          forall (vs1 vs2 : list val) (j : nat) (t1 : type) 
-            (xs1 : list var) (e1 : exp) (rho1' : env),
-            length vs1 = length vs2 ->
-            find_def f1 defs1 = Some (t1, xs1, e1) ->
-            Some rho1' = setlist xs1 vs1 (def_funs defs1 defs1 rho1 rho1) ->
-            exists (t2 : type) (Γ : var) (xs2 : list var) (e2 : exp) (rho2' : env),
-              find_def f2 defs2 = Some (t2, Γ :: xs2, e2) /\
-              Some rho2' = setlist (Γ :: xs2) ((Vconstr tau' t' fvs) :: vs2)
-                                   (def_funs defs2 defs2 rho2 rho2) /\
-              match k with
-                | 0 => True
-                | S k =>
-                  let R := cc_approx_val (k - (k-j)) in
-                  j < S k ->
-                  Forall2 R vs1 vs2 ->
-                  cc_approx_exp (k - (k - j)) (e1, rho1') (e2, rho2')
-              end
-        | Vconstr tau1 t1 vs1, Vconstr tau2 t2 vs2 =>
-          t1 = t2 /\ Forall2_aux vs1 vs2
-        | Vint n1, Vint n2 => n1 = n2
-        | _, _ => False
-      end
-  in cc_approx_val_aux v1 v2.
+  Fixpoint cc_approx_val (k : nat) (v1 v2 : val) {struct k} : Prop :=
+    let cc_approx_exp (k : nat) (p1 p2 : exp * env) : Prop :=
+        let '(e1, rho1) := p1 in
+        let '(e2, rho2) := p2 in
+        forall v1 c1,
+          c1 <= k -> bstep_e pr cenv rho1 e1 v1 c1 ->
+          exists v2 c2, bstep_e pr cenv rho2 e2 v2 c2 /\ 
+                   cc_approx_val (k - c1) v1 v2
+    in
+    let fix cc_approx_val_aux (v1 v2 : val) {struct v1} : Prop :=
+        let fix Forall2_aux vs1 vs2 :=
+            match vs1, vs2 with
+              | [], _ => True
+              | v1 :: vs1, v2 :: vs2 =>
+                cc_approx_val_aux v1 v2 /\ Forall2_aux vs1 vs2
+              | _, _ => False
+            end
+        in
+        match v1, v2 with
+          | Vfun rho1 defs1 f1,
+            Vconstr tag ((Vfun rho2 defs2 f2) ::  (Vconstr tag' fvs) :: l)  =>
+            forall (vs1 vs2 : list val) (j : nat) (t : fTag) 
+              (xs1 : list var) (e1 : exp) (rho1' : env),
+              length vs1 = length vs2 ->
+              find_def f1 defs1 = Some (t, xs1, e1) ->
+              Some rho1' = setlist xs1 vs1 (def_funs defs1 defs1 rho1 rho1) ->
+              exists (Γ : var) (xs2 : list var) (e2 : exp) (rho2' : env),
+                tag = clo_tag /\
+                find_def f2 defs2 = Some (t, Γ :: xs2, e2) /\              
+                Some rho2' = setlist (Γ :: xs2) ((Vconstr tag' fvs) :: vs2)
+                                     (def_funs defs2 defs2 rho2 rho2) /\
+                match k with
+                  | 0 => True
+                  | S k =>
+                    let R := cc_approx_val (k - (k-j)) in
+                    j < S k ->
+                    Forall2 R vs1 vs2 ->
+                    cc_approx_exp (k - (k - j)) (e1, rho1') (e2, rho2')
+                end
+          | Vconstr t1 vs1, Vconstr t2 vs2 =>
+            t1 = t2 /\ Forall2_aux vs1 vs2
+          | Vint n1, Vint n2 => n1 = n2
+          | _, _ => False
+        end
+    in cc_approx_val_aux v1 v2.
 
-Definition cc_approx_exp (k : nat) (p1 p2 : exp * env) : Prop :=
-  let '(e1, rho1) := p1 in
-  let '(e2, rho2) := p2 in
-  forall v1 c1,
-    c1 <= k -> bstep_e pr rho1 e1 v1 c1 ->
-    exists v2 c2, bstep_e pr rho2 e2 v2 c2 /\
-             cc_approx_val (k - c1) v1 v2.
+  Definition cc_approx_exp (k : nat) (p1 p2 : exp * env) : Prop :=
+    let '(e1, rho1) := p1 in
+    let '(e2, rho2) := p2 in
+    forall v1 c1,
+      c1 <= k -> bstep_e pr cenv rho1 e1 v1 c1 ->
+      exists v2 c2, bstep_e pr cenv rho2 e2 v2 c2 /\
+               cc_approx_val (k - c1) v1 v2.
 
-(** more compact definition of the value relation *)
-Definition cc_approx_val' (k : nat) (v1 v2 : val) : Prop :=
-  match v1, v2 with
-    | Vfun rho1 defs1 f1,
-      Vconstr tau t ((Vfun rho2 defs2 f2) ::  (Vconstr tau' t' fvs) :: l) =>
-      forall (vs1 vs2 : list val) (j : nat) (t1 : type) 
-        (xs1 : list var) (e1 : exp) (rho1' : env),
-        length vs1 = length vs2 ->
-        find_def f1 defs1 = Some (t1, xs1, e1) ->
-        Some rho1' = setlist xs1 vs1 (def_funs defs1 defs1 rho1 rho1) ->
-        exists (t2 : type) (Γ : var) (xs2 : list var) (e2 : exp) (rho2' : env),
-          find_def f2 defs2 = Some (t2, Γ :: xs2, e2) /\
-          Some rho2' = setlist (Γ :: xs2) ((Vconstr tau' t' fvs) :: vs2)
-                               (def_funs defs2 defs2 rho2 rho2) /\
-          (j < k -> Forall2 (cc_approx_val j) vs1 vs2 ->
-           cc_approx_exp j (e1, rho1') (e2, rho2'))
-    | Vconstr tau1 t1 vs1, Vconstr tau2 t2 vs2 =>
-      t1 = t2 /\ Forall2_asym (cc_approx_val k) vs1 vs2
-    | Vint n1, Vint n2 => n1 = n2
-    | _, _ => False
-  end.
+  (** More compact definition of the value relation *)
+  Definition cc_approx_val' (k : nat) (v1 v2 : val) : Prop :=
+    match v1, v2 with
+      | Vfun rho1 defs1 f1,
+        Vconstr tag ((Vfun rho2 defs2 f2) ::  (Vconstr tag' fvs) :: l) =>
+        forall (vs1 vs2 : list val) (j : nat) (t : fTag) 
+          (xs1 : list var) (e1 : exp) (rho1' : env),
+          length vs1 = length vs2 ->
+          find_def f1 defs1 = Some (t, xs1, e1) ->
+          Some rho1' = setlist xs1 vs1 (def_funs defs1 defs1 rho1 rho1) ->
+          exists (Γ : var) (xs2 : list var) (e2 : exp) (rho2' : env),
+            tag = clo_tag /\
+            find_def f2 defs2 = Some (t, Γ :: xs2, e2) /\
+            Some rho2' = setlist (Γ :: xs2) ((Vconstr tag' fvs) :: vs2)
+                                 (def_funs defs2 defs2 rho2 rho2) /\
+            (j < k -> Forall2 (cc_approx_val j) vs1 vs2 ->
+             cc_approx_exp j (e1, rho1') (e2, rho2'))
+      | Vconstr t1 vs1, Vconstr t2 vs2 =>
+        t1 = t2 /\ Forall2_asym (cc_approx_val k) vs1 vs2
+      | Vint n1, Vint n2 => n1 = n2
+      | _, _ => False
+    end.
 
-(** correspondence of the two definitions *)
-Lemma cc_approx_val_eq (k : nat) (v1 v2 : val) :
-  cc_approx_val k v1 v2 <-> cc_approx_val' k v1 v2.
-Proof.
-  destruct k as [ | k ]; destruct v1; destruct v2;
-  eauto; try (split; intros H; (now simpl in H; inv H)).
-  - split.
-    * revert l0; induction l as [| x xs IHxs];
-      intros l2; destruct l2 as [| y ys ];
-      try (now intros [H1 H2]; split; eauto; inv H2).
-      intros H; split; destruct H as [H1 [H2 H3]]; eauto.
-      constructor; [ now eauto | now eapply IHxs ].
-    * revert l0; induction l as [| x xs IHxs];
-      intros l2; destruct l2 as [| y ys ];
-      try (now intros [H1 H2]; split; eauto; inv H2).
-      intros H; split; inv H; eauto. inv H1.
-      split; [ now eauto | now eapply IHxs ].
-  - split; intros Hpre; simpl; destruct l; try contradiction;
-    destruct v0; try contradiction; destruct l; try contradiction;
-    destruct l; try contradiction; destruct v1; try contradiction;
-    intros; edestruct (Hpre vs1 vs2 0) as [t2' [Γ [xs2 [e2 [rho' [H1' [H2' H3']]]]]]];
-    eauto; do 5 eexists; repeat split; eauto; intros Hc; exfalso; omega.
-  - split.
-    * revert l0; induction l as [| x xs IHxs];
-      intros l2; destruct l2 as [| y ys ];
-      try (now intros [H1 H2]; split; eauto; inv H2).
-      intros H; split; destruct H as [H1 [H2 H3]]; eauto. constructor. eauto.
-      eapply IHxs. simpl. eauto.
-    * revert l0; induction l as [| x xs IHxs];
-      intros l2; destruct l2 as [| y ys ];
-      try (now intros [H1 H2]; split; eauto; inv H2).
-      intros H; split; inv H; eauto. inv H1.
-      split; [now eauto | now apply IHxs].
-  - split; intros Hpre; simpl; destruct l; try contradiction;
-    destruct v0; try contradiction; destruct l; try contradiction;
-    destruct l; try contradiction; destruct v1; try contradiction;
-    intros;
-    edestruct (Hpre vs1 vs2 j) as [t2' [Γ [xs2 [e2 [rho' [H1' [H2' H3']]]]]]];
-    eauto; do 5 eexists; repeat split; eauto; intros Hleq Hf v1 c1 Hleq' Hstep;
-    (assert (Heq : k - (k - j) = j) by omega);
-    rewrite Heq in *;  eapply H3'; eauto.
-Qed.
+  (** Correspondence of the two definitions *)
+  Lemma cc_approx_val_eq (k : nat) (v1 v2 : val) :
+    cc_approx_val k v1 v2 <-> cc_approx_val' k v1 v2.
+  Proof.
+    destruct k as [ | k ]; destruct v1; destruct v2;
+    eauto; try (split; intros H; (now simpl in H; inv H)).
+    - split.
+      * revert l0; induction l as [| x xs IHxs];
+        intros l2; destruct l2 as [| y ys ];
+        try (now intros [H1 H2]; split; eauto; inv H2).
+        intros H; split; destruct H as [H1 [H2 H3]]; eauto.
+        constructor; [ now eauto | now eapply IHxs ].
+      * revert l0; induction l as [| x xs IHxs];
+        intros l2; destruct l2 as [| y ys ];
+        try (now intros [H1 H2]; split; eauto; inv H2).
+        intros H; split; inv H; eauto. inv H1.
+        split; [ now eauto | now eapply IHxs ].
+    - split; intros Hpre; simpl; destruct l; try contradiction;
+      destruct v0; try contradiction; destruct l; try contradiction;
+      destruct l; try contradiction; destruct v1; try contradiction;
+      intros; edestruct (Hpre vs1 vs2 0) as [Γ [xs2 [e2 [rho' [Heq [H1' [H2' H3']]]]]]];
+      eauto; subst; do 4 eexists; repeat split; eauto; intros Hc; exfalso; omega.
+    - split.
+      * revert l0; induction l as [| x xs IHxs];
+        intros l2; destruct l2 as [| y ys ];
+        try (now intros [H1 H2]; split; eauto; inv H2).
+        intros H; split; destruct H as [H1 [H2 H3]]; eauto. constructor. eauto.
+        eapply IHxs. simpl. eauto.
+      * revert l0; induction l as [| x xs IHxs];
+        intros l2; destruct l2 as [| y ys ];
+        try (now intros [H1 H2]; split; eauto; inv H2).
+        intros H; split; inv H; eauto. inv H1.
+        split; [now eauto | now apply IHxs].
+    - split; intros Hpre; simpl; destruct l; try contradiction;
+      destruct v0; try contradiction; destruct l; try contradiction;
+      destruct l; try contradiction; destruct v1; try contradiction;
+      intros;
+      edestruct (Hpre vs1 vs2 j) as [Γ [xs2 [e2 [rho' [Heq [H1' [H2' H3']]]]]]];
+      eauto; do 4 eexists; repeat split; eauto; intros Hleq Hf v1 c1 Hleq' Hstep;
+      (assert (Heq' : k - (k - j) = j) by omega);
+      rewrite Heq' in *;  eapply H3'; eauto.
+  Qed.
 
-Opaque cc_approx_val.
+  Opaque cc_approx_val.
 
-(** Environment relation for a single point (i.e. variable) : 
- * ρ1 ~_k^x ρ2 iff ρ1(x) = Some v -> ρ2(x) = Some v' /\ v ~_k v' *)
-Definition cc_approx_var_env (k : nat) (rho1 rho2 : env) (x y : var) : Prop :=
-  forall v1, 
-    M.get x rho1 = Some v1 -> 
-    exists v2, M.get y rho2 = Some v2 /\ cc_approx_val k v1 v2.
+  (** Environment relation for a single point (i.e. variable) : 
+   * ρ1 ~_k^x ρ2 iff ρ1(x) = Some v -> ρ2(x) = Some v' /\ v ~_k v' *)
+  Definition cc_approx_var_env (k : nat) (rho1 rho2 : env) (x y : var) : Prop :=
+    forall v1, 
+      M.get x rho1 = Some v1 -> 
+      exists v2, M.get y rho2 = Some v2 /\ cc_approx_val k v1 v2.
 
-(** Environment relation for a set of points (i.e. predicate over variables) : 
- * ρ1 ~_k^S ρ2 iff 
- *   forall x, S x -> ρ1(x) = Some v -> ρ2(x) = Some v' /\ v ~_k v' *)
-Definition cc_approx_env_P (P : Ensemble var) k rho1 rho2 :=
-  forall (x : var), P x -> cc_approx_var_env k rho1 rho2 x x.
+  (** Environment relation for a set of points (i.e. predicate over variables) : 
+   * ρ1 ~_k^S ρ2 iff 
+   *   forall x, S x -> ρ1(x) = Some v -> ρ2(x) = Some v' /\ v ~_k v' *)
+  Definition cc_approx_env_P (P : Ensemble var) k rho1 rho2 :=
+    forall (x : var), P x -> cc_approx_var_env k rho1 rho2 x x.
 
-(** Environment relation for the whole domain of definition :
- * ρ1 ~_k ρ2 iff forall x, ρ1(x) = v => ρ2(x) = v' /\ v ~_k v' *)
-Definition cc_approx_env (k : nat) (rho1 rho2 : env) : Prop :=
-  cc_approx_env_P (fun _ => True) k rho1 rho2.
+  (** Environment relation for the whole domain of definition :
+   * ρ1 ~_k ρ2 iff forall x, ρ1(x) = v => ρ2(x) = v' /\ v ~_k v' *)
+  Definition cc_approx_env (k : nat) (rho1 rho2 : env) : Prop :=
+    cc_approx_env_P (fun _ => True) k rho1 rho2.
 
-(** Lemmas about extending the environment *)
-Lemma cc_approx_var_env_extend_eq :
-  forall (rho1 rho2 : env) (k : nat) (x : var) (v1 v2 : val),
-    cc_approx_val k v1 v2 ->
-    cc_approx_var_env k (M.set x v1 rho1) (M.set x v2 rho2) x x.
-Proof.
-  intros rho1 rho2 k x v1 v2 Hval x' Hget.
-  rewrite M.gss in Hget. inv Hget. eexists. rewrite M.gss. split; eauto.
-Qed.
+  (** Lemmas about extending the environment *)
+  Lemma cc_approx_var_env_extend_eq :
+    forall (rho1 rho2 : env) (k : nat) (x : var) (v1 v2 : val),
+      cc_approx_val k v1 v2 ->
+      cc_approx_var_env k (M.set x v1 rho1) (M.set x v2 rho2) x x.
+  Proof.
+    intros rho1 rho2 k x v1 v2 Hval x' Hget.
+    rewrite M.gss in Hget. inv Hget. eexists. rewrite M.gss. split; eauto.
+  Qed.
 
-Lemma cc_approx_var_env_extend_neq :
-  forall (rho1 rho2 : env) (k : nat) (x y : var) (v1 v2 : val),
-    cc_approx_var_env k rho1 rho2 y y ->
-    y <> x ->
-    cc_approx_var_env k (M.set x v1 rho1) (M.set x v2 rho2) y y.
-Proof.
-  intros rho1 rho2 k x  y v1 v2 Hval Hneq x' Hget.
-  rewrite M.gso in *; eauto.
-Qed.
+  Lemma cc_approx_var_env_extend_neq :
+    forall (rho1 rho2 : env) (k : nat) (x y : var) (v1 v2 : val),
+      cc_approx_var_env k rho1 rho2 y y ->
+      y <> x ->
+      cc_approx_var_env k (M.set x v1 rho1) (M.set x v2 rho2) y y.
+  Proof.
+    intros rho1 rho2 k x  y v1 v2 Hval Hneq x' Hget.
+    rewrite M.gso in *; eauto.
+  Qed.
 
-Lemma cc_approx_var_env_extend :
-  forall (rho1 rho2 : env) (k : nat) (x y : var) (v1 v2 : val),
-    cc_approx_var_env k rho1 rho2 y y ->
-    cc_approx_val k v1 v2 ->
-    cc_approx_var_env k (M.set x v1 rho1) (M.set x v2 rho2) y y.
-Proof.
-  intros rho1 rho2 k x y v1 v2 Henv Hval.
-  destruct (Coqlib.peq y x); subst.
-  - apply cc_approx_var_env_extend_eq; eauto.
-  - apply cc_approx_var_env_extend_neq; eauto.
-Qed.
+  Lemma cc_approx_var_env_extend :
+    forall (rho1 rho2 : env) (k : nat) (x y : var) (v1 v2 : val),
+      cc_approx_var_env k rho1 rho2 y y ->
+      cc_approx_val k v1 v2 ->
+      cc_approx_var_env k (M.set x v1 rho1) (M.set x v2 rho2) y y.
+  Proof.
+    intros rho1 rho2 k x y v1 v2 Henv Hval.
+    destruct (Coqlib.peq y x); subst.
+    - apply cc_approx_var_env_extend_eq; eauto.
+    - apply cc_approx_var_env_extend_neq; eauto.
+  Qed.
 
-(** The environment relation is antimonotonic in the set
- * of free variables *) 
-Lemma cc_approx_env_P_antimon (P1 P2 : var -> Prop) k rho1 rho2 :
-  cc_approx_env_P P2 k rho1 rho2 ->
-  (Included var P1 P2) ->
-  cc_approx_env_P P1 k rho1 rho2.
-Proof.
-  intros Hpre Hin x HP2. eapply Hpre; eapply Hin; eauto.
-Qed.
+  (** The environment relation is antimonotonic in the set
+   * of free variables *) 
+  Lemma cc_approx_env_P_antimon (P1 P2 : var -> Prop) k rho1 rho2 :
+    cc_approx_env_P P2 k rho1 rho2 ->
+    (Included var P1 P2) ->
+    cc_approx_env_P P1 k rho1 rho2.
+  Proof.
+    intros Hpre Hin x HP2. eapply Hpre; eapply Hin; eauto.
+  Qed.
 
-Global Instance cc_approx_env_proper :
-  Proper (Same_set var ==> Logic.eq ==> Logic.eq ==> Logic.eq ==> iff)
-         cc_approx_env_P.
-Proof.
-  intros s1 s2 [H1 H2]; split; intros Hpre;
-  eapply cc_approx_env_P_antimon; subst; eauto.
-Qed.
+  Global Instance cc_approx_env_proper :
+    Proper (Same_set var ==> Logic.eq ==> Logic.eq ==> Logic.eq ==> iff)
+           cc_approx_env_P.
+  Proof.
+    intros s1 s2 [H1 H2]; split; intros Hpre;
+    eapply cc_approx_env_P_antimon; subst; eauto.
+  Qed.
 
-(** Lemmas about the sets that index the environment relation *)
-Lemma cc_approx_env_Empty_set k (rho1 rho2 : env) :
-  cc_approx_env_P (Empty_set var) k rho1 rho2.
-Proof.
-  intros x H. inv H.
-Qed.
+  (** Lemmas about the sets that index the environment relation *)
+  Lemma cc_approx_env_Empty_set k (rho1 rho2 : env) :
+    cc_approx_env_P (Empty_set var) k rho1 rho2.
+  Proof.
+    intros x H. inv H.
+  Qed.
 
-Lemma cc_approx_env_P_union (P1 P2 : var -> Prop) k rho1 rho2 :
-  cc_approx_env_P P1 k rho1 rho2 ->
-  cc_approx_env_P P2 k rho1 rho2 ->
-  cc_approx_env_P (Union var P1 P2) k rho1 rho2.
-Proof.
-  intros Hpre1 Hpre2 x HP2. inv HP2; eauto.
-Qed.
-
-Lemma cc_approx_env_P_inter_l (P1 P2 : var -> Prop) k rho1 rho2 :
-  cc_approx_env_P P1 k rho1 rho2 ->
-  cc_approx_env_P (Intersection var P1 P2) k rho1 rho2.
-Proof.
-  intros Hpre x HP2. inv HP2; eauto.
-Qed.
-
-Lemma cc_approx_env_P_inter_r (P1 P2 : var -> Prop) k rho1 rho2 :
-  cc_approx_env_P P2 k rho1 rho2 ->
-  cc_approx_env_P (Intersection var P1 P2) k rho1 rho2.
-Proof.
-  intros Hpre x HP2.
-  inv HP2; eauto.
-Qed.
-
-(** Extend the related environments with a single point *)
-Lemma cc_approx_env_P_extend :
-  forall P (rho1 rho2 : env) (k : nat) (x : var) (v1 v2 : val),
-    cc_approx_env_P (Setminus var P (Singleton var x)) k rho1 rho2 ->
-    cc_approx_val k v1 v2 ->
-    cc_approx_env_P P k (M.set x v1 rho1) (M.set x v2 rho2).
-Proof.
-  intros P rho1 rho2 k x v1 v2 Henv Hval x' HP v1' Hget.
-  rewrite M.gsspec in Hget. destruct (Coqlib.peq x' x); subst.
-  - inv Hget. eexists. rewrite M.gss. split; eauto.
-  - apply Henv in Hget; eauto. destruct Hget as [v2' [Heq Hpre]].
-    eexists; split; eauto. rewrite M.gso; eauto. constructor; eauto.
-    intros Hin. inv Hin. congruence.
-Qed.
-
-(** Extend the related environments with a list *)
-Lemma cc_approx_env_P_setlist_l:
-  forall (P1 P2 : var -> Prop) (rho1 rho2 rho1' rho2' : env)
-    (k : nat) (xs : list var) (vs1 vs2 : list val),
+  Lemma cc_approx_env_P_union (P1 P2 : var -> Prop) k rho1 rho2 :
     cc_approx_env_P P1 k rho1 rho2 ->
-    (forall x, ~ List.In x xs -> P2 x -> P1 x) ->
+    cc_approx_env_P P2 k rho1 rho2 ->
+    cc_approx_env_P (Union var P1 P2) k rho1 rho2.
+  Proof.
+    intros Hpre1 Hpre2 x HP2. inv HP2; eauto.
+  Qed.
+
+  Lemma cc_approx_env_P_inter_l (P1 P2 : var -> Prop) k rho1 rho2 :
+    cc_approx_env_P P1 k rho1 rho2 ->
+    cc_approx_env_P (Intersection var P1 P2) k rho1 rho2.
+  Proof.
+    intros Hpre x HP2. inv HP2; eauto.
+  Qed.
+
+  Lemma cc_approx_env_P_inter_r (P1 P2 : var -> Prop) k rho1 rho2 :
+    cc_approx_env_P P2 k rho1 rho2 ->
+    cc_approx_env_P (Intersection var P1 P2) k rho1 rho2.
+  Proof.
+    intros Hpre x HP2.
+    inv HP2; eauto.
+  Qed.
+
+  (** Extend the related environments with a single point *)
+  Lemma cc_approx_env_P_extend :
+    forall P (rho1 rho2 : env) (k : nat) (x : var) (v1 v2 : val),
+      cc_approx_env_P (Setminus var P (Singleton var x)) k rho1 rho2 ->
+      cc_approx_val k v1 v2 ->
+      cc_approx_env_P P k (M.set x v1 rho1) (M.set x v2 rho2).
+  Proof.
+    intros P rho1 rho2 k x v1 v2 Henv Hval x' HP v1' Hget.
+    rewrite M.gsspec in Hget. destruct (Coqlib.peq x' x); subst.
+    - inv Hget. eexists. rewrite M.gss. split; eauto.
+    - apply Henv in Hget; eauto. destruct Hget as [v2' [Heq Hpre]].
+      eexists; split; eauto. rewrite M.gso; eauto. constructor; eauto.
+      intros Hin. inv Hin. congruence.
+  Qed.
+
+  (** Extend the related environments with a list *)
+  Lemma cc_approx_env_P_setlist_l:
+    forall (P1 P2 : var -> Prop) (rho1 rho2 rho1' rho2' : env)
+      (k : nat) (xs : list var) (vs1 vs2 : list val),
+      cc_approx_env_P P1 k rho1 rho2 ->
+      (forall x, ~ List.In x xs -> P2 x -> P1 x) ->
+      Forall2 (cc_approx_val k) vs1 vs2 ->
+      setlist xs vs1 rho1 = Some rho1' ->
+      setlist xs vs2 rho2 = Some rho2' ->
+      cc_approx_env_P P2 k rho1' rho2'.
+  Proof.
+    intros P1 P2 rho1' rho2' rho1 rho2 k xs vs1 vs2 Hpre Hyp Hall Hset1 Hset2
+           x HP v Hget.
+    destruct (in_dec var_dec x xs).
+    - edestruct setlist_Forall2_get as [v1 [v2 [Hget1 [Hget2 HP']]]]; eauto.
+      rewrite Hget in Hget1. inv Hget1. repeat eexists; eauto.
+    - erewrite <- setlist_not_In in Hget; eauto.
+      edestruct Hpre as [v2 [Hget' Hpre']]; eauto.
+      repeat eexists; eauto. erewrite <- setlist_not_In; eauto.
+  Qed.
+
+
+  Lemma cc_approx_var_env_getlist (rho1 rho2 : env) (k : nat)
+        (xs ys : list var) (vs1 : list val) :
+    Forall2 (cc_approx_var_env k rho1 rho2) xs ys ->
+    getlist xs rho1 = Some vs1 ->
+    exists vs2,
+      getlist ys rho2 = Some vs2 /\ Forall2 (cc_approx_val k) vs1 vs2.
+  Proof.
+    revert ys vs1. induction xs as [| x xs IHxs]; intros ys vs2 Hall Hget.
+    - destruct ys; inv Hall. inv Hget. eexists. split; simpl; eauto.
+    - simpl in Hget.
+      destruct (M.get x rho1) eqn:Heq1; try discriminate.
+      destruct (getlist xs rho1) eqn:Heq2; try discriminate. inv Hget.
+      destruct ys as [| y ys]; inv Hall. 
+      destruct (IHxs ys l H4 eq_refl) as [vs2 [Hget HAll]].
+      destruct (H2 _ Heq1) as [v2 [Heq Hpre]].
+      eexists. split; simpl; eauto. rewrite Hget, Heq. eauto.
+  Qed.
+
+  Lemma cc_approx_env_P_getlist_l (P : var -> Prop) (rho1 rho2 : env) (k : nat)
+        (xs : list var) (vs1 : list val) :
+    cc_approx_env_P P k rho1 rho2 ->
+    Included _ (FromList xs) P ->
+    getlist xs rho1 = Some vs1 ->
+    exists vs2,
+      getlist xs rho2 = Some vs2 /\ Forall2 (cc_approx_val k) vs1 vs2.
+  Proof.
+    intros Henv. revert vs1.
+    induction xs as [| x xs IHxs]; intros vs1 Hp Hget.
+    - inv Hget. eexists. split; simpl; eauto.
+    - simpl in Hget. destruct (M.get x rho1) eqn:Heq1; try discriminate.
+      destruct (getlist xs rho1) eqn:Heq2; try discriminate. inv Hget.
+      edestruct (IHxs l) as  [vs2 [Hget HAll]]; eauto.
+      + intros x' Hin. eapply Hp. constructor 2; eauto.
+      + eapply Henv in Heq1. destruct Heq1 as [v2 [H1 H2]].
+        eexists. split; simpl; eauto. rewrite H1. rewrite Hget.
+        constructor. apply Hp. now constructor.
+  Qed.
+
+  Corollary cc_approx_env_getlist_l (rho1 rho2 : env) (k : nat)
+            (xs : list var) (vs1 : list val) :
+    cc_approx_env k rho1 rho2 ->
+    getlist xs rho1 = Some vs1 ->
+    exists vs2,
+      getlist xs rho2 = Some vs2 /\ Forall2 (cc_approx_val k) vs1 vs2.
+  Proof.
+    intros. eapply cc_approx_env_P_getlist_l; eauto.
+    intros x H'; simpl; eauto.
+  Qed.
+
+  Corollary cc_approx_env_extend (rho1 rho2 : env) (k : nat)
+            (x : var) (v1 v2 : val) :
+    cc_approx_env k rho1 rho2 ->
+    cc_approx_val k v1 v2 ->
+    cc_approx_env k (M.set x v1 rho1) (M.set x v2 rho2).
+  Proof.
+    intros H1 Hval. apply cc_approx_env_P_extend; eauto.
+    eapply cc_approx_env_P_antimon; eauto. intros x' H; simpl; eauto.
+  Qed.
+
+  Corollary cc_approx_env_setlist_l (rho1 rho2 rho1' rho2' : env) (k : nat)
+            (xs : list var) (vs1 vs2 : list val) :
+    cc_approx_env k rho1 rho2 ->
     Forall2 (cc_approx_val k) vs1 vs2 ->
     setlist xs vs1 rho1 = Some rho1' ->
     setlist xs vs2 rho2 = Some rho2' ->
-    cc_approx_env_P P2 k rho1' rho2'.
-Proof.
-  intros P1 P2 rho1' rho2' rho1 rho2 k xs vs1 vs2 Hpre Hyp Hall Hset1 Hset2
-         x HP v Hget.
-  destruct (in_dec var_dec x xs).
-  - edestruct setlist_Forall2_get as [v1 [v2 [Hget1 [Hget2 HP']]]]; eauto.
-    rewrite Hget in Hget1. inv Hget1. repeat eexists; eauto.
-  - erewrite <- setlist_not_In in Hget; eauto.
-    edestruct Hpre as [v2 [Hget' Hpre']]; eauto.
-    repeat eexists; eauto. erewrite <- setlist_not_In; eauto.
-Qed.
+    cc_approx_env k rho1' rho2'.
+  Proof.
+    intros. eapply cc_approx_env_P_setlist_l; eauto.
+  Qed.
+
+  Lemma cc_approx_env_P_set_not_in_P_r P k rho rho' x v :
+    cc_approx_env_P P k rho rho' ->
+    ~ In _ P x ->
+    cc_approx_env_P P k rho (M.set x v rho').
+  Proof. 
+    intros Hcc Hnin y Py v' Hget.
+    edestruct Hcc as [v'' [Hget' Happrox]]; eauto.
+    exists v''. rewrite M.gsspec.
+    destruct (Coqlib.peq y x); subst.
+    - contradiction.
+    - eauto.
+  Qed.
+
+  Lemma cc_approx_env_P_def_funs_not_In_P_l k rho1 rho2 S B B' :
+    Disjoint _ S (name_in_fundefs B') ->
+    cc_approx_env_P S k rho1 rho2 ->
+    cc_approx_env_P S k (def_funs B B' rho1 rho1) rho2.
+  Proof.
+    intros Hd Hcc x HS v Hget. eapply Hcc; eauto. 
+    erewrite <- def_funs_neq. eassumption.  
+    intros Hc. eapply Hd; constructor; eauto.
+  Qed.
+
+  Lemma cc_approx_env_P_def_funs_not_In_P_r k rho1 rho2 S B B' :
+    Disjoint _ S (name_in_fundefs B') ->
+    cc_approx_env_P S k rho1 rho2 ->
+    cc_approx_env_P S k rho1 (def_funs B B' rho2 rho2).
+  Proof.
+    intros Hd Hcc x HS v Hget.
+    edestruct Hcc as [v' [Hget' Hcc']]; eauto.
+    eexists; split; eauto.
+    rewrite def_funs_neq. eassumption.
+    intros Hc. eapply Hd; constructor; eauto.
+  Qed.
+
+  (** * Index Monotonicity Properties *)
+
+  (** The value relation is monotonic in the step index *)
+  Lemma cc_approx_val_monotonic (k : nat) :
+    (forall v1 v2 j,
+       cc_approx_val k v1 v2 -> j <= k -> cc_approx_val j v1 v2).
+  Proof.
+    intros v1 v2 h Hpre Hleq. try rewrite cc_approx_val_eq in *.
+    revert v2 Hpre; induction v1 using val_ind'; intros v2 Hpre;
+    destruct v2; try (simpl; contradiction); eauto.
+    - destruct l; try now inv Hpre.
+    - inv Hpre. inv H0.
+      split; auto. constructor; rewrite cc_approx_val_eq in *.
+      now eapply IHv1; eauto.
+      destruct (IHv0 ((Vconstr c l'))) as [Heq Hpre']; eauto.
+      now split; eauto.
+    - destruct l; try contradiction. destruct v0; try contradiction. 
+      destruct l; try contradiction. destruct v1; try contradiction. 
+      intros vs1 vs2 j t1' xs e1 rho1' Hlen Hf Heq.
+      edestruct Hpre as [Γ [xs2 [e2 [rho2' [Heq' [H1 [H2 H3]]]]]]]; eauto.
+      subst. do 4 eexists; repeat split; eauto. intros Hleq' Hall.
+      eapply H3; eauto. omega.
+  Qed.
+
+  (** The expression relation is monotonic in the step index *)
+  Lemma cc_approx_exp_monotonic (k : nat) :
+    (forall rho1 e1 rho2 e2 j,
+       cc_approx_exp k (rho1, e1) (rho2, e2) ->
+       j <= k -> cc_approx_exp j (rho1, e1) (rho2, e2)).
+  Proof.
+    intros rho1 e1 rho2 e2 j Hpre Hleq v1 c1 Hlt Hstep.
+    edestruct (Hpre v1 c1) as [v2 [c2 [H1 H2]]]; eauto. omega.
+    do 2 eexists; split; eauto.
+    eapply cc_approx_val_monotonic. eapply H2. omega.
+  Qed.
+
+  (** The environment relations are monotonic in the step index *)
+  Lemma cc_approx_env_P_monotonic :
+    forall P (k j : nat) (rho1 rho2 : env),
+      j <= k -> cc_approx_env_P P k rho1 rho2 -> cc_approx_env_P P j rho1 rho2.
+  Proof.
+    intros P k j rho1 rho2 Hleq Hpre x HP v Hget.
+    edestruct Hpre as [v2 [Heq Hpre2]]; eauto.
+    eexists; split; eauto. eapply cc_approx_val_monotonic; eauto.
+  Qed.
+
+  Lemma cc_approx_env_monotonic k j rho1 rho2 :
+    j <= k -> cc_approx_env k rho1 rho2 -> cc_approx_env j rho1 rho2.
+  Proof.
+    intros Hleq H. eapply cc_approx_env_P_monotonic; eauto.
+  Qed.
 
 
-Lemma cc_approx_var_env_getlist (rho1 rho2 : env) (k : nat)
-      (xs ys : list var) (vs1 : list val) :
-  Forall2 (cc_approx_var_env k rho1 rho2) xs ys ->
-  getlist xs rho1 = Some vs1 ->
-  exists vs2,
-    getlist ys rho2 = Some vs2 /\ Forall2 (cc_approx_val k) vs1 vs2.
-Proof.
-  revert ys vs1. induction xs as [| x xs IHxs]; intros ys vs2 Hall Hget.
-  - destruct ys; inv Hall. inv Hget. eexists. split; simpl; eauto.
-  - simpl in Hget.
-    destruct (M.get x rho1) eqn:Heq1; try discriminate.
-    destruct (getlist xs rho1) eqn:Heq2; try discriminate. inv Hget.
-    destruct ys as [| y ys]; inv Hall. 
-    destruct (IHxs ys l H4 eq_refl) as [vs2 [Hget HAll]].
-    destruct (H2 _ Heq1) as [v2 [Heq Hpre]].
-    eexists. split; simpl; eauto. rewrite Hget, Heq. eauto.
-Qed.
+  (** * Compatibility lemmas *)
 
-Lemma cc_approx_env_P_getlist_l (P : var -> Prop) (rho1 rho2 : env) (k : nat)
-      (xs : list var) (vs1 : list val) :
-  cc_approx_env_P P k rho1 rho2 ->
-  Included _ (FromList xs) P ->
-  getlist xs rho1 = Some vs1 ->
-  exists vs2,
-    getlist xs rho2 = Some vs2 /\ Forall2 (cc_approx_val k) vs1 vs2.
-Proof.
-  intros Henv. revert vs1.
-  induction xs as [| x xs IHxs]; intros vs1 Hp Hget.
-  - inv Hget. eexists. split; simpl; eauto.
-  - simpl in Hget. destruct (M.get x rho1) eqn:Heq1; try discriminate.
-    destruct (getlist xs rho1) eqn:Heq2; try discriminate. inv Hget.
-    edestruct (IHxs l) as  [vs2 [Hget HAll]]; eauto.
-    + intros x' Hin. eapply Hp. constructor 2; eauto.
-    + eapply Henv in Heq1. destruct Heq1 as [v2 [H1 H2]].
-      eexists. split; simpl; eauto. rewrite H1. rewrite Hget.
-      constructor. apply Hp. now constructor.
-Qed.
+  Lemma cc_approx_exp_const_compat k rho1 rho2 x t ys1 ys2 e1 e2 :
+    Forall2 (cc_approx_var_env k rho1 rho2) ys1 ys2 ->
+    (forall vs1 vs2 : list val,
+       Forall2 (cc_approx_val k) vs1 vs2 ->
+       cc_approx_exp k (e1, M.set x (Vconstr t vs1) rho1)
+                     (e2, M.set x (Vconstr t vs2) rho2)) ->
+    cc_approx_exp k (Econstr x t ys1 e1, rho1) (Econstr x t ys2 e2, rho2).
+  Proof.
+    intros Hall Hpre v1 c1 Hleq1 Hstep1. inv Hstep1.
+    edestruct (cc_approx_var_env_getlist rho1 rho2) as [vs2' [Hget' Hpre']];
+      [| eauto |]; eauto.
+    edestruct Hpre as [v2 [c2 [Hstep Hval]]]; eauto.
+    repeat eexists; eauto. econstructor; eauto.
+  Qed.
 
-Corollary cc_approx_env_getlist_l (rho1 rho2 : env) (k : nat)
-          (xs : list var) (vs1 : list val) :
-  cc_approx_env k rho1 rho2 ->
-  getlist xs rho1 = Some vs1 ->
-  exists vs2,
-    getlist xs rho2 = Some vs2 /\ Forall2 (cc_approx_val k) vs1 vs2.
-Proof.
-  intros. eapply cc_approx_env_P_getlist_l; eauto.
-  intros x H'; simpl; eauto.
-Qed.
+  Lemma cc_approx_exp_proj_compat k rho1 rho2 x tau n y1 y2 e1 e2 :
+    cc_approx_var_env k rho1 rho2 y1 y2 ->
+    (forall v1 v2,
+       cc_approx_val k v1 v2 -> 
+       cc_approx_exp k (e1, M.set x v1 rho1)
+                     (e2, M.set x v2 rho2)) ->
+    cc_approx_exp k (Eproj x tau n y1 e1, rho1) (Eproj x tau n y2 e2, rho2).
+  Proof.
+    intros Henv Hexp v1 c1 Hleq1 Hstep1. inv Hstep1.
+    edestruct Henv as [v' [Hget Hpre]]; eauto.
+    destruct v'; rewrite cc_approx_val_eq in Hpre; simpl in Hpre; try contradiction.
+    inv Hpre.
+    edestruct (Forall2_asym_nthN (cc_approx_val k) vs l) as [v2 [Hnth Hval]]; eauto.
+    edestruct Hexp as [v2' [c2 [Hstep Hval']]]; eauto.
+    repeat eexists; eauto. econstructor; eauto.
+  Qed.
 
-Corollary cc_approx_env_extend (rho1 rho2 : env) (k : nat)
-          (x : var) (v1 v2 : val) :
-  cc_approx_env k rho1 rho2 ->
-  cc_approx_val k v1 v2 ->
-  cc_approx_env k (M.set x v1 rho1) (M.set x v2 rho2).
-Proof.
-  intros H1 Hval. apply cc_approx_env_P_extend; eauto.
-  eapply cc_approx_env_P_antimon; eauto. intros x' H; simpl; eauto.
-Qed.
+  Lemma cc_approx_exp_case_nil_compat k rho1 rho2 x1 x2 :
+    cc_approx_exp k (Ecase x1 [], rho1) (Ecase x2 [], rho2).
+  Proof.
+    intros v1 c1 Hleq1 Hstep1. inv Hstep1. inv H4.
+  Qed.
 
-Corollary cc_approx_env_setlist_l (rho1 rho2 rho1' rho2' : env) (k : nat)
-          (xs : list var) (vs1 vs2 : list val) :
-  cc_approx_env k rho1 rho2 ->
-  Forall2 (cc_approx_val k) vs1 vs2 ->
-  setlist xs vs1 rho1 = Some rho1' ->
-  setlist xs vs2 rho2 = Some rho2' ->
-  cc_approx_env k rho1' rho2'.
-Proof.
-  intros. eapply cc_approx_env_P_setlist_l; eauto.
-Qed.
+  Lemma cc_approx_exp_case_cons_compat k rho1 rho2 x1 x2 c e1 e2 P1 P2:
+    Forall2 (fun p1 p2 => fst p1 = fst p2) P1 P2 ->
+    cc_approx_var_env k rho1 rho2 x1 x2 ->
+    cc_approx_exp k (e1, rho1) (e2, rho2) ->
+    cc_approx_exp k (Ecase x1 P1, rho1)
+                  (Ecase x2 P2, rho2) ->
+    cc_approx_exp k (Ecase x1 ((c, e1) :: P1), rho1)
+                  (Ecase x2 ((c, e2) :: P2), rho2).
+  Proof.
+    intros Hall Henv Hexp_hd Hexp_tl v1 c1 Hleq1 Hstep1. inv Hstep1. inv H4.
+    destruct (M.elt_eq c t) eqn:Heq; subst.
+    - inv H0. edestruct Hexp_hd as [v2 [c2 [Hstep2 Hpre2]]]; eauto.
+      edestruct Henv as [v2' [Hget Hpre]]; eauto.
+      rewrite cc_approx_val_eq in Hpre.
+      destruct v2'; try (now simpl in Hpre; contradiction). inv Hpre. 
+      repeat eexists; eauto. econstructor; eauto; [| now simpl; rewrite Heq; eauto ].
+      inv H2. econstructor; eauto. eapply caseConsistent_same_cTags; eassumption.
+    - edestruct Hexp_tl as [v2 [c2 [Hstep2 Hpre2]]]; eauto. inv H2.
+      econstructor; eauto. inv Hstep2.
+      edestruct Henv as [v2' [Hget Hpre]]; eauto.
+      rewrite cc_approx_val_eq in Hpre.
+      destruct v2'; try (now simpl in Hpre; contradiction). inv Hpre.
+      rewrite Hget in H4; inv H4.
+      repeat eexists; eauto. econstructor; eauto; [| now simpl; rewrite Heq; eauto ].
+      inv H2. econstructor; eauto.
+  Qed.
 
-Lemma cc_approx_env_P_set_not_in_P_r P k rho rho' x v :
-  cc_approx_env_P P k rho rho' ->
-  ~ In _ P x ->
-  cc_approx_env_P P k rho (M.set x v rho').
-Proof. 
-  intros Hcc Hnin y Py v' Hget.
-  edestruct Hcc as [v'' [Hget' Happrox]]; eauto.
-  exists v''. rewrite M.gsspec.
-  destruct (Coqlib.peq y x); subst.
-  - contradiction.
-  - eauto.
-Qed.
+  Axiom Prim_axiom_cc :
+    forall f f' v1,
+      M.get f pr = Some f' ->
+      forall k vs1 vs2,
+        Forall2 (cc_approx_val k) vs1 vs2 ->
+        f' vs1 = Some v1 ->
+        exists v2,
+          f' vs2 = Some v2 /\                      
+          cc_approx_val k v1 v2.
 
-Lemma cc_approx_env_P_def_funs_not_In_P_l k rho1 rho2 S B B' :
-  Disjoint _ S (name_in_fundefs B') ->
-  cc_approx_env_P S k rho1 rho2 ->
-  cc_approx_env_P S k (def_funs B B' rho1 rho1) rho2.
-Proof.
-  intros Hd Hcc x HS v Hget. eapply Hcc; eauto. 
-  erewrite <- def_funs_neq. eassumption.  
-  intros Hc. eapply Hd; constructor; eauto.
-Qed.
+  Lemma cc_approx_exp_prim_compat k rho1 rho2 x1 x2 f ys1 ys2 e1 e2 :
+    Forall2 (cc_approx_var_env k rho1 rho2) ys1 ys2 ->
+    (forall v1 v2,
+       cc_approx_val k v1 v2 -> 
+       cc_approx_exp k (e1, M.set x1 v1 rho1)
+                     (e2, M.set x2 v2 rho2)) ->
+    cc_approx_exp k (Eprim x1 f ys1 e1, rho1) (Eprim x2 f ys2 e2, rho2).
+  Proof.
+    intros Henv Hexp v1 c1 Hleq1 Hstep1. inv Hstep1.
+    edestruct cc_approx_var_env_getlist as [vs2 [Hget' Hpre']]; eauto.
+    edestruct Prim_axiom_cc as [v2 [Heq Hprev2]]; eauto.
+    edestruct Hexp as [v2' [c2 [Hstepv2' Hprev2']]]; eauto.
+    repeat eexists; eauto. econstructor; eauto.
+  Qed.
 
-Lemma cc_approx_env_P_def_funs_not_In_P_r k rho1 rho2 S B B' :
-  Disjoint _ S (name_in_fundefs B') ->
-  cc_approx_env_P S k rho1 rho2 ->
-  cc_approx_env_P S k rho1 (def_funs B B' rho2 rho2).
-Proof.
-  intros Hd Hcc x HS v Hget.
-  edestruct Hcc as [v' [Hget' Hcc']]; eauto.
-  eexists; split; eauto.
-  rewrite def_funs_neq. eassumption.
-  intros Hc. eapply Hd; constructor; eauto.
-Qed.
+  (** Lift a value predicate to a subset of an environment *)
+  Definition lift_P_env (S : Ensemble var) (P : Ensemble val) (rho : env) :=
+    forall x v, S x -> M.get x rho = Some v -> P v.
 
-(** * Index Monotonicity Properties *)
+  Lemma lift_P_env_antimon S S' P rho :
+    Included _ S S' ->
+    lift_P_env S' P rho ->
+    lift_P_env S P rho.
+  Proof.
+    intros H Henv x v HS Hget.
+    eapply Henv; eauto. eapply H; eauto.
+  Qed.
 
-(** The value relation is monotonic in the step index *)
-Lemma cc_approx_val_monotonic (k : nat) :
-  (forall v1 v2 j,
-     cc_approx_val k v1 v2 -> j <= k -> cc_approx_val j v1 v2).
-Proof.
-  intros v1 v2 h Hpre Hleq. try rewrite cc_approx_val_eq in *.
-  revert v2 Hpre; induction v1 using val_ind'; intros v2 Hpre;
-  destruct v2; try (simpl; contradiction); eauto.
-  - destruct l; try now inv Hpre.
-  - inv Hpre. inv H0.
-    split; auto. constructor; rewrite cc_approx_val_eq in *.
-    now eapply IHv1; eauto.
-    destruct (IHv0 ((Vconstr tau t1 l'))) as [Heq Hpre']; eauto.
-    now split; eauto.
-  - destruct l; try contradiction. destruct v0; try contradiction. 
-    destruct l; try contradiction. destruct v1; try contradiction. 
-    intros vs1 vs2 j t1' xs e1 rho1' Hlen Hf Heq.
-    edestruct Hpre as [t2' [Γ [xs2 [e2 [rho2' [H1 [H2 H3]]]]]]]; eauto.
-    do 5 eexists; split; eauto. split; eauto. intros Hleq' Hall. 
-    eapply H3; eauto. omega.
-Qed.
+  Global Instance lift_P_env_proper : Proper (Same_set var ==> eq ==> eq ==> iff) lift_P_env.
+  Proof.
+    intros S1 S2 Heq P1 P2 Heq' rho1 rho2 Heq''; subst.
+    split; intros H x v Hs Hget; (eapply H; [ | now eauto ]);
+    now eapply Heq.
+  Qed.
 
-(** The expression relation is monotonic in the step index *)
-Lemma cc_approx_exp_monotonic (k : nat) :
-  (forall rho1 e1 rho2 e2 j,
-     cc_approx_exp k (rho1, e1) (rho2, e2) ->
-     j <= k -> cc_approx_exp j (rho1, e1) (rho2, e2)).
-Proof.
-  intros rho1 e1 rho2 e2 j Hpre Hleq v1 c1 Hlt Hstep.
-  edestruct (Hpre v1 c1) as [v2 [c2 [H1 H2]]]; eauto. omega.
-  do 2 eexists; split; eauto.
-  eapply cc_approx_val_monotonic. eapply H2. omega.
-Qed.
+  Lemma lift_P_env_Union_l S1 S2 P rho :
+    lift_P_env (Union _ S1 S2) P rho ->
+    lift_P_env S1 P rho.
+  Proof.
+    intros H. eapply lift_P_env_antimon; [| now eauto ].
+    now apply Included_Union_l.
+  Qed.
 
-(** The environment relations are monotonic in the step index *)
-Lemma cc_approx_env_P_monotonic :
-  forall P (k j : nat) (rho1 rho2 : env),
-    j <= k -> cc_approx_env_P P k rho1 rho2 -> cc_approx_env_P P j rho1 rho2.
-Proof.
-  intros P k j rho1 rho2 Hleq Hpre x HP v Hget.
-  edestruct Hpre as [v2 [Heq Hpre2]]; eauto.
-  eexists; split; eauto. eapply cc_approx_val_monotonic; eauto.
-Qed.
+  Lemma lift_P_env_Union_r S1 S2 P rho :
+    lift_P_env (Union _ S1 S2) P rho ->
+    lift_P_env S2 P rho.
+  Proof.
+    intros H. eapply lift_P_env_antimon; [| now eauto ].
+    now apply Included_Union_r.
+  Qed.
 
-Lemma cc_approx_env_monotonic k j rho1 rho2 :
-  j <= k -> cc_approx_env k rho1 rho2 -> cc_approx_env j rho1 rho2.
-Proof.
-  intros Hleq H. eapply cc_approx_env_P_monotonic; eauto.
-Qed.
+  Lemma lift_P_env_Emtpy_set P rho :
+    lift_P_env (Empty_set _) P rho.
+  Proof.
+    intros x v H. inv H.
+  Qed.
 
 
-(** * Compatibility lemmas *)
+  Lemma lift_P_env_extend S P rho x v :
+    lift_P_env (Setminus _ S (Singleton _ x)) P rho ->
+    P v ->
+    lift_P_env S P (M.set x v rho). 
+  Proof.
+    intros H Hp x' v' HS Hget.
+    rewrite M.gsspec in Hget.
+    destruct (Coqlib.peq x' x); subst.
+    - now inv Hget.
+    - eapply H; [| eassumption ].
+      constructor; eauto. intros Hc. inv Hc. congruence.
+  Qed.
 
-Lemma cc_approx_exp_const_compat k rho1 rho2 x tau t ys1 ys2 e1 e2 :
-  Forall2 (cc_approx_var_env k rho1 rho2) ys1 ys2 ->
-  (forall vs1 vs2 : list val,
-     Forall2 (cc_approx_val k) vs1 vs2 ->
-     cc_approx_exp k (e1, M.set x (Vconstr tau t vs1) rho1)
-                   (e2, M.set x (Vconstr tau t vs2) rho2)) ->
-  cc_approx_exp k (Econstr x tau t ys1 e1, rho1) (Econstr x tau t ys2 e2, rho2).
-Proof.
-  intros Hall Hpre v1 c1 Hleq1 Hstep1. inv Hstep1.
-  edestruct (cc_approx_var_env_getlist rho1 rho2) as [vs2' [Hget' Hpre']];
-    [| eauto |]; eauto.
-  edestruct Hpre as [v2 [c2 [Hstep Hval]]]; eauto.
-  repeat eexists; eauto. econstructor; eauto.
-Qed.
+  Lemma lift_P_env_setlist S P rho rho' xs vs :
+    lift_P_env (Setminus _ S (FromList xs)) P rho ->
+    Forall P vs ->
+    setlist xs vs rho = Some rho' ->
+    lift_P_env S P rho'. 
+  Proof.
+    revert S xs rho rho'. induction vs; intros S xs rho rho' Henv Hall Hset.
+    - destruct xs; inv Hset.
+      rewrite FromList_nil, Setminus_Empty_set_Same_set in Henv.
+      eapply Henv; now eauto.
+    - destruct xs; try discriminate. inv Hall.
+      simpl in Hset. destruct (setlist xs vs rho) eqn:Heq ; try discriminate.
+      inv Hset. eapply lift_P_env_extend; eauto.
+      eapply IHvs; eauto.
+      now rewrite FromList_cons, <- Setminus_Union in Henv.
+  Qed.
 
-Lemma cc_approx_exp_proj_compat k rho1 rho2 x tau n y1 y2 e1 e2 :
-  cc_approx_var_env k rho1 rho2 y1 y2 ->
-  (forall v1 v2,
-     cc_approx_val k v1 v2 -> 
-     cc_approx_exp k (e1, M.set x v1 rho1)
-                   (e2, M.set x v2 rho2)) ->
-  cc_approx_exp k (Eproj x tau n y1 e1, rho1) (Eproj x tau n y2 e2, rho2).
-Proof.
-  intros Henv Hexp v1 c1 Hleq1 Hstep1. inv Hstep1.
-  edestruct Henv as [v' [Hget Hpre]]; eauto.
-  destruct v'; rewrite cc_approx_val_eq in Hpre; simpl in Hpre; try contradiction.
-  inv Hpre.
-  edestruct (Forall2_asym_nthN (cc_approx_val k) vs l) as [v2 [Hnth Hval]]; eauto.
-  edestruct Hexp as [v2' [c2 [Hstep Hval']]]; eauto.
-  repeat eexists; eauto. econstructor; eauto.
-Qed.
+  Lemma lift_P_env_def_funs S P B B' rho  :
+    lift_P_env (Setminus _ S (name_in_fundefs B)) P rho ->
+    (forall f, P (Vfun rho B' f)) ->
+    lift_P_env S P (def_funs B' B rho rho). 
+  Proof.
+    revert S rho. induction B; intros S rho Henv Hfun.
+    - simpl. eapply lift_P_env_extend; [| now eauto ].
+      eapply IHB; [| eassumption ].
+      eapply lift_P_env_antimon; [| eassumption ].
+      rewrite Setminus_Union. now eapply Included_refl.
+    - now rewrite Setminus_Empty_set_Same_set in Henv. 
+  Qed.
 
-Lemma cc_approx_exp_case_nil_compat k rho1 rho2 x1 x2 :
-  cc_approx_exp k (Ecase x1 [], rho1) (Ecase x2 [], rho2).
-Proof.
-  intros v1 c1 Hleq1 Hstep1. inv Hstep1. inv H3.
-Qed.
+  Lemma lift_P_env_get S P rho x v :
+    lift_P_env S P rho ->
+    Included _ (Singleton _ x) S ->
+    M.get x rho = Some v ->
+    P v.
+  Proof.
+    intros Henv HS Hget. eapply Henv; eauto. 
+    now eapply HS; eauto. 
+  Qed.
 
-Lemma cc_approx_exp_case_cons_compat k rho1 rho2 x1 x2 c e1 e2 P1 P2:
-  cc_approx_var_env k rho1 rho2 x1 x2 ->
-  cc_approx_exp k (e1, rho1) (e2, rho2) ->
-  cc_approx_exp k (Ecase x1 P1, rho1)
-                (Ecase x2 P2, rho2) ->
-  cc_approx_exp k (Ecase x1 ((c, e1) :: P1), rho1)
-                (Ecase x2 ((c, e2) :: P2), rho2).
-Proof.
-  intros Henv Hexp_hd Hexp_tl v1 c1 Hleq1 Hstep1. inv Hstep1. inv H3.
-  destruct (M.elt_eq c t) eqn:Heq; subst.
-  - inv H0. edestruct Hexp_hd as [v2 [c2 [Hstep2 Hpre2]]]; eauto.
-    edestruct Henv as [v2' [Hget Hpre]]; eauto.
-    rewrite cc_approx_val_eq in Hpre.
-    destruct v2'; try (now simpl in Hpre; contradiction). inv Hpre. 
-    repeat eexists; eauto. econstructor; eauto. simpl; rewrite Heq; eauto.
-  - edestruct Hexp_tl as [v2 [c2 [Hstep2 Hpre2]]]; eauto.
-    econstructor; eauto. inv Hstep2.
-    edestruct Henv as [v2' [Hget Hpre]]; eauto.
-    rewrite cc_approx_val_eq in Hpre.
-    destruct v2'; try (now simpl in Hpre; contradiction). inv Hpre.
-    rewrite Hget in H3; inv H3.
-    repeat eexists; eauto. econstructor; eauto. simpl; rewrite Heq; eauto.
-Qed.
+  Lemma lift_P_env_getlist S P rho xs vs :
+    lift_P_env S P rho ->
+    Included _ (FromList xs) S ->
+    getlist xs rho = Some vs ->
+    Forall P vs.
+  Proof.
+    revert S xs rho. induction vs; intros S xs rho Henv Hincl Hget.
+    - eauto.
+    - destruct xs; try discriminate. simpl in Hget.
+      destruct (M.get v rho) eqn:Heq; try discriminate.
+      destruct (getlist xs rho) eqn:Heq'; try discriminate.
+      inv Hget. rewrite FromList_cons in Hincl.
+      constructor.
+      + eapply lift_P_env_get; eauto.
+        eapply Included_trans; [| now eauto ].
+        eapply Included_Union_l.
+      + eapply IHvs; eauto.
+        eapply Included_trans; [| now eauto ].
+        eapply Included_Union_r.
+  Qed.
 
-Axiom Prim_axiom_cc :
-  forall f f' v1,
-    M.get f pr = Some f' ->
-    forall k vs1 vs2,
-      Forall2 (cc_approx_val k) vs1 vs2 ->
-      f' vs1 = Some v1 ->
-      exists v2,
-        f' vs2 = Some v2 /\                      
-        cc_approx_val k v1 v2.
+  Lemma Forall_nthN {A} (R : A -> Prop) l n v :
+    Forall R l ->
+    nthN l n = Some v ->
+    R v.
+  Proof.
+    revert n. induction l; intros n Hall Hnth; [ discriminate |].
+    inv Hall. simpl in Hnth.
+    destruct n. 
+    - inv Hnth; eauto.
+    - eapply IHl; eauto.  
+  Qed. 
 
-Lemma cc_approx_exp_prim_compat k rho1 rho2 x1 x2 tau f ys1 ys2 e1 e2 :
-  Forall2 (cc_approx_var_env k rho1 rho2) ys1 ys2 ->
-  (forall v1 v2,
-     cc_approx_val k v1 v2 -> 
-     cc_approx_exp k (e1, M.set x1 v1 rho1)
-                   (e2, M.set x2 v2 rho2)) ->
-  cc_approx_exp k (Eprim x1 tau f ys1 e1, rho1) (Eprim x2 tau f ys2 e2, rho2).
-Proof.
-  intros Henv Hexp v1 c1 Hleq1 Hstep1. inv Hstep1.
-  edestruct cc_approx_var_env_getlist as [vs2 [Hget' Hpre']]; eauto.
-  edestruct Prim_axiom_cc as [v2 [Heq Hprev2]]; eauto.
-  edestruct Hexp as [v2' [c2 [Hstepv2' Hprev2']]]; eauto.
-  repeat eexists; eauto. econstructor; eauto.
-Qed.
+  
+  Lemma cc_approx_exp_respects_preord_exp_r_pre (k : nat)
+        (rho1 rho2 rho3 : env) (e1 e2 e3 : exp) :
+    (forall j v1 v2 v3,
+       j <= k ->
+       cc_approx_val j v1 v2 ->
+       (forall k, preord_val k v2 v3) ->
+       cc_approx_val j v1 v3) ->
+    cc_approx_exp k (e1, rho1) (e2, rho2) ->
+    (forall k', preord_exp k' (e2, rho2) (e3, rho3)) ->
+    cc_approx_exp k (e1, rho1) (e3, rho3).
+  Proof.
+    intros IH Hexp1 Hexp2 v1 c Hleq1 Hstep1. 
+    edestruct Hexp1 as [v2 [c2 [Hstep2 Hpre2]]]; eauto. 
+    edestruct (Hexp2 c2) as [v3 [c3 [Hstep3 Hpre3]]]; [| eauto | ]. omega.
+    exists v3, c3. split; eauto.
+    eapply IH; [ omega | now eauto | ].
+    intros m.
+    edestruct (Hexp2 (m + c2)) as [v3' [c3' [Hstep3' Hpre3']]]; [| eauto |]. omega.
+    eapply bstep_e_deterministic in Hstep3; eauto. inv Hstep3.
+    eapply preord_val_monotonic; eauto. omega.
+  Qed.
 
-(** Lift a value predicate to a subset of an environment *)
-Definition lift_P_env (S : Ensemble var) (P : Ensemble val) (rho : env) :=
-  forall x v, S x -> M.get x rho = Some v -> P v.
+  Lemma occurs_free_closed_fundefs f tau xs e B :
+    fun_in_fundefs B (f, tau, xs, e) ->
+    closed_fundefs B ->
+    Included _ (occurs_free e) (Union _ (FromList xs) (name_in_fundefs B)).
+  Proof.
+    intros H Hcl.
+    eapply Included_trans. now eapply occurs_free_in_fun; eauto.
+    unfold closed_fundefs in Hcl. rewrite Hcl, Union_Empty_set_l.
+    eapply Included_refl.
+  Qed.
 
-Lemma lift_P_env_antimon S S' P rho :
-  Included _ S S' ->
-  lift_P_env S' P rho ->
-  lift_P_env S P rho.
-Proof.
-  intros H Henv x v HS Hget.
-  eapply Henv; eauto. eapply H; eauto.
-Qed.
+  Lemma cc_approx_val_respects_preord_val_r (k : nat) (v1 v2 v3 : val) :
+    cc_approx_val k v1 v2 ->
+    (forall k, preord_val k v2 v3) ->
+    cc_approx_val k v1 v3.
+  Proof.
+    revert v1 v2 v3. induction k using lt_wf_rec.
+    induction v1 using val_ind'; intros v2 v3 Happrox Hpre;
+    assert (Hpre' := Hpre k);
+    rewrite cc_approx_val_eq, preord_val_eq in *.
+    - destruct v2; try contradiction.
+      destruct v3; try contradiction.
+      inv Hpre'; inv Happrox. split; eauto.
+    - destruct v2; try contradiction.
+      destruct v3; try contradiction.
+      destruct l0; [now inv Happrox; inv H1 |].
+      destruct l1; [now inv Hpre'; inv H1 |].
+      inv Hpre'; inv Happrox. inv H1; inv H2; split; eauto.
+      constructor; eauto.
+      + eapply IHv1; [ now eauto |].
+        intros k'. specialize (Hpre k').
+        rewrite preord_val_eq in Hpre. inv Hpre. now inv H1.
+      + assert (Hsuf : cc_approx_val' k (Vconstr c0 l) (Vconstr c0 l1)).
+        { rewrite <- cc_approx_val_eq.
+          eapply IHv0 with (v2 := Vconstr c0 l0).
+          - rewrite cc_approx_val_eq. now split; eauto.
+          - intros k'. specialize (Hpre k'). rewrite preord_val_eq in Hpre.
+            inv Hpre. inv H1. rewrite preord_val_eq. now split; eauto. }
+        now inv Hsuf.
+    - destruct v2, v3; try contradiction. 
+      destruct l; try contradiction.
+      destruct v0, l; try contradiction.
+      destruct v1; try contradiction. 
+      inversion Hpre' as [Hleq Hall]. clear Hpre'. inv Hall.
+      rewrite preord_val_eq in H2. inv H4.
+      rewrite preord_val_eq in H3.
+      destruct y, y0; try contradiction.
+      intros vs1 vs2 j t1' xs1 e1 rho1 Heq1 Hfind1 Hset1.
+      edestruct (Happrox vs1 vs2) as [Γ [xs2 [e2 [rho2' [Heq [Hfind2 [Hset2 Heval2]]]]]]]; eauto.
+      subst.
+      edestruct (H2 (Vconstr c1 l1 :: vs2) (Vconstr c l0 :: vs2)) with (j := 0) as
+          [xs3' [e3 [rho3 [Hfind3 [Hset3 _]]]]]; eauto.
+      edestruct xs3' as [| Γ' xs3]; try discriminate. 
+      do 4 eexists. repeat split; eauto.
+      intros Hlt Hall. 
+      eapply cc_approx_exp_respects_preord_exp_r_pre
+      with (e2 := e2) (rho2 := rho2').
+      + intros. eapply H; [ omega | eassumption | eassumption ].
+      + eapply Heval2. omega. assumption.
+      + intros k'. specialize (Hpre (k'+1)). rewrite preord_val_eq in Hpre.
+        inversion Hpre as [_ Hall']. clear Hpre. inv Hall'.
+        rewrite preord_val_eq in H5. 
+        edestruct (H5 (Vconstr c1 l1 :: vs2) (Vconstr c l0 :: vs2)) as
+            [xs3'' [e3' [rho4 [Hfind3' [Hset3' Heval3']]]]]; eauto. 
+        rewrite Hfind3' in Hfind3. inv Hfind3.
+        rewrite <- Hset3 in Hset3'. inv Hset3'.
+        eapply Heval3'. omega. inv H8. constructor.
+        eapply preord_val_monotonic. eassumption. omega.
+        eapply Forall2_refl. eapply preord_val_refl.
+    - destruct v2; try contradiction.
+      destruct v3; try contradiction. inv Happrox.
+      inv Hpre'. reflexivity.
+  Qed.
 
-Instance lift_P_env_proper : Proper (Same_set var ==> eq ==> eq ==> iff) lift_P_env.
-Proof.
-  intros S1 S2 Heq P1 P2 Heq' rho1 rho2 Heq''; subst.
-  split; intros H x v Hs Hget; (eapply H; [ | now eauto ]);
-  now eapply Heq.
-Qed.
+  (* The following are obsolete *)
+  (* TODO: move to identifiers.v *)
+  Inductive closed_fundefs_in_val : val -> Prop :=
+  | Vconstr_closed :
+      forall t vs,
+        Forall closed_fundefs_in_val vs ->
+        closed_fundefs_in_val (Vconstr t vs)
+  | Vfun_closed :
+      forall rho B f,
+        closed_fundefs B ->
+        closed_fundefs_in_fundefs B ->
+        (* fun_in_fundefs B (f, tau, xs, e) -> *)
+        (* Included _ (occurs_free e) (Union _ (FromList xs) (name_in_fundefs B)) -> *)
+        closed_fundefs_in_val (Vfun rho B f)
+  | Vint_closed :
+      forall z, closed_fundefs_in_val (Vint z).
 
-Lemma lift_P_env_Union_l S1 S2 P rho :
-  lift_P_env (Union _ S1 S2) P rho ->
-  lift_P_env S1 P rho.
-Proof.
-  intros H. eapply lift_P_env_antimon; [| now eauto ].
-  now apply Included_Union_l.
-Qed.
+  Definition closed_fundefs_in_env (S : Ensemble var) rho : Prop :=
+    lift_P_env S closed_fundefs_in_val rho.
 
-Lemma lift_P_env_Union_r S1 S2 P rho :
-  lift_P_env (Union _ S1 S2) P rho ->
-  lift_P_env S2 P rho.
-Proof.
-  intros H. eapply lift_P_env_antimon; [| now eauto ].
-  now apply Included_Union_r.
-Qed.
+  Lemma fun_in_fundefs_funs_in_fundef B B' f t xs e :
+    fun_in_fundefs B (f, t, xs, e) ->
+    funs_in_exp B' e ->
+    funs_in_fundef B' B.
+  Proof.
+    induction B; intros Hin Hfuns.
+    - inv Hin.
+      + inv H. now eauto.
+      + constructor 2. eapply IHB; eauto.
+    - inv Hin.
+  Qed.
 
-Lemma lift_P_env_Emtpy_set P rho :
-  lift_P_env (Empty_set _) P rho.
-Proof.
-  intros x v H. inv H.
-Qed.
-
-
-Lemma lift_P_env_extend S P rho x v :
-  lift_P_env (Setminus _ S (Singleton _ x)) P rho ->
-  P v ->
-  lift_P_env S P (M.set x v rho). 
-Proof.
-  intros H Hp x' v' HS Hget.
-  rewrite M.gsspec in Hget.
-  destruct (Coqlib.peq x' x); subst.
-  - now inv Hget.
-  - eapply H; [| eassumption ].
-    constructor; eauto. intros Hc. inv Hc. congruence.
-Qed.
-
-Lemma lift_P_env_setlist S P rho rho' xs vs :
-  lift_P_env (Setminus _ S (FromList xs)) P rho ->
-  Forall P vs ->
-  setlist xs vs rho = Some rho' ->
-  lift_P_env S P rho'. 
-Proof.
-  revert S xs rho rho'. induction vs; intros S xs rho rho' Henv Hall Hset.
-  - destruct xs; inv Hset.
-    rewrite FromList_nil, Setminus_Empty_set_Same_set in Henv.
-    eapply Henv; now eauto.
-  - destruct xs; try discriminate. inv Hall.
-    simpl in Hset. destruct (setlist xs vs rho) eqn:Heq ; try discriminate.
-    inv Hset. eapply lift_P_env_extend; eauto.
-    eapply IHvs; eauto.
-    now rewrite FromList_cons, <- Setminus_Union in Henv.
-Qed.
-
-Lemma lift_P_env_def_funs S P B B' rho  :
-  lift_P_env (Setminus _ S (name_in_fundefs B)) P rho ->
-  (forall f, P (Vfun rho B' f)) ->
-  lift_P_env S P (def_funs B' B rho rho). 
-Proof.
-  revert S rho. induction B; intros S rho Henv Hfun.
-  - simpl. eapply lift_P_env_extend; [| now eauto ].
-    eapply IHB; [| eassumption ].
-    eapply lift_P_env_antimon; [| eassumption ].
-    rewrite Setminus_Union. now eapply Included_refl.
-  - now rewrite Setminus_Empty_set_Same_set in Henv. 
-Qed.
-
-Lemma lift_P_env_get S P rho x v :
-  lift_P_env S P rho ->
-  Included _ (Singleton _ x) S ->
-  M.get x rho = Some v ->
-  P v.
-Proof.
-  intros Henv HS Hget. eapply Henv; eauto. 
-  now eapply HS; eauto. 
-Qed.
-
-Lemma lift_P_env_getlist S P rho xs vs :
-  lift_P_env S P rho ->
-  Included _ (FromList xs) S ->
-  getlist xs rho = Some vs ->
-  Forall P vs.
-Proof.
-  revert S xs rho. induction vs; intros S xs rho Henv Hincl Hget.
-  - eauto.
-  - destruct xs; try discriminate. simpl in Hget.
-    destruct (M.get v rho) eqn:Heq; try discriminate.
-    destruct (getlist xs rho) eqn:Heq'; try discriminate.
-    inv Hget. rewrite FromList_cons in Hincl.
-    constructor.
-    + eapply lift_P_env_get; eauto.
-      eapply Included_trans; [| now eauto ].
-      eapply Included_Union_l.
-    + eapply IHvs; eauto.
-      eapply Included_trans; [| now eauto ].
-      eapply Included_Union_r.
-Qed.
-
-Lemma Forall_nthN {A} (R : A -> Prop) l n v :
-  Forall R l ->
-  nthN l n = Some v ->
-  R v.
-Proof.
-  revert n. induction l; intros n Hall Hnth; [ discriminate |].
-  inv Hall. simpl in Hnth.
-  destruct n. 
-  - inv Hnth; eauto.
-  - eapply IHl; eauto.  
-Qed. 
-
- 
-Lemma cc_approx_exp_respects_preord_exp_r_pre (k : nat)
-      (rho1 rho2 rho3 : env) (e1 e2 e3 : exp) :
-  (forall j v1 v2 v3,
-     j <= k ->
-     cc_approx_val j v1 v2 ->
-     (forall k, preord_val k v2 v3) ->
-     cc_approx_val j v1 v3) ->
-  cc_approx_exp k (e1, rho1) (e2, rho2) ->
-  (forall k', preord_exp k' (e2, rho2) (e3, rho3)) ->
-  cc_approx_exp k (e1, rho1) (e3, rho3).
-Proof.
-  intros IH Hexp1 Hexp2 v1 c Hleq1 Hstep1. 
-  edestruct Hexp1 as [v2 [c2 [Hstep2 Hpre2]]]; eauto. 
-  edestruct (Hexp2 c2) as [v3 [c3 [Hstep3 Hpre3]]]; [| eauto | ]. omega.
-  exists v3, c3. split; eauto.
-  eapply IH; [ omega | now eauto | ].
-  intros m.
-  edestruct (Hexp2 (m + c2)) as [v3' [c3' [Hstep3' Hpre3']]]; [| eauto |]. omega.
-  eapply bstep_e_deterministic in Hstep3; eauto. inv Hstep3.
-  eapply preord_val_monotonic; eauto. omega.
-Qed.
-
-Lemma occurs_free_closed_fundefs f tau xs e B :
-  fun_in_fundefs B (f, tau, xs, e) ->
-  closed_fundefs B ->
-  Included _ (occurs_free e) (Union _ (FromList xs) (name_in_fundefs B)).
-Proof.
-  intros H Hcl.
-  eapply Included_trans. now eapply occurs_free_in_fun; eauto.
-  unfold closed_fundefs in Hcl. rewrite Hcl, Union_Empty_set_l.
-  eapply Included_refl.
-Qed.
-
-Lemma cc_approx_val_respects_preord_val_r (k : nat) (v1 v2 v3 : val) :
-  cc_approx_val k v1 v2 ->
-  (forall k, preord_val k v2 v3) ->
-  cc_approx_val k v1 v3.
-Proof.
-  revert v1 v2 v3. induction k using lt_wf_rec.
-  induction v1 using val_ind'; intros v2 v3 Happrox Hpre;
-  assert (Hpre' := Hpre k);
-  rewrite cc_approx_val_eq, preord_val_eq in *.
-  - destruct v2; try contradiction.
-    destruct v3; try contradiction.
-    inv Hpre'; inv Happrox. split; eauto.
-  - destruct v2; try contradiction.
-    destruct v3; try contradiction.
-    destruct l0; [now inv Happrox; inv H1 |].
-    destruct l1; [now inv Hpre'; inv H1 |].
-    inv Hpre'; inv Happrox. inv H1; inv H2; split; eauto.
-    constructor; eauto.
-    + eapply IHv1; [ now eauto |].
-      intros k'. specialize (Hpre k').
-      rewrite preord_val_eq in Hpre. inv Hpre. now inv H1.
-    + assert (Hsuf : cc_approx_val' k (Vconstr tau t3 l)  (Vconstr tau t3 l1)).
-      { rewrite <- cc_approx_val_eq.
-        eapply IHv0 with (v2 := Vconstr tau t3 l0).
-        - rewrite cc_approx_val_eq. now split; eauto.
-        - intros k'. specialize (Hpre k'). rewrite preord_val_eq in Hpre.
-          inv Hpre. inv H1. rewrite preord_val_eq. now split; eauto. }
-      now inv Hsuf.
-  - destruct v2, v3; try contradiction. 
-    destruct l; try contradiction.
-    destruct v0, l; try contradiction.
-    destruct v1; try contradiction. 
-    inversion Hpre' as [Hleq Hall]. clear Hpre'. inv Hall.
-    rewrite preord_val_eq in H2. inv H4.
-    rewrite preord_val_eq in H3.
-    destruct y, y0; try contradiction.
-    intros vs1 vs2 j t1' xs1 e1 rho1 Heq1 Hfind1 Hset1.
-    edestruct (Happrox vs1 vs2) as [t2' [Γ [xs2 [e2 [rho2' [Hfind2 [Hset2 Heval2]]]]]]]; eauto.
-    edestruct (H2 (Vconstr t5 t6 l1 :: vs2) (Vconstr t7 t8 l0 :: vs2)) with (j := 0) as
-        [t3' [xs3' [e3 [rho3 [Hfind3 [Hset3 _]]]]]]; eauto.
-    edestruct xs3' as [| Γ' xs3]; try discriminate. 
-    do 5 eexists. repeat split; eauto.
-    intros Hlt Hall. 
-    eapply cc_approx_exp_respects_preord_exp_r_pre
-    with (e2 := e2) (rho2 := rho2').
-    + intros. eapply H; [ omega | eassumption | eassumption ].
-    + eapply Heval2. omega. assumption.
-    + intros k'. specialize (Hpre (k'+1)). rewrite preord_val_eq in Hpre.
-      inversion Hpre as [_ Hall']. clear Hpre. inv Hall'.
-      rewrite preord_val_eq in H5.
-      edestruct (H5 (Vconstr t5 t6 l1 :: vs2) (Vconstr t7 t8 l0 :: vs2)) as
-          [t3'' [xs3'' [e3' [rho4 [Hfind3' [Hset3' Heval3']]]]]]; eauto. 
-      rewrite Hfind3' in Hfind3. inv Hfind3.
-      rewrite <- Hset3 in Hset3'. inv Hset3'.
-      eapply Heval3'. omega. inv H8. constructor.
-      eapply preord_val_monotonic. eassumption. omega.
-      eapply Forall2_refl. eapply preord_val_refl.
-  - destruct v2; try contradiction.
-    destruct v3; try contradiction. inv Happrox.
-    inv Hpre'. reflexivity.
-Qed.
-
-(* The following are obsolete *)
-(* TODO: move to identifiers.v *)
-Inductive closed_fundefs_in_val : val -> Prop :=
-| Vconstr_closed :
-    forall tau t vs,
+  Axiom prims_closed_fundefs :
+    forall (f : prim) (f' : list val -> option val) vs v,
+      M.get f pr = Some f' ->
       Forall closed_fundefs_in_val vs ->
-      closed_fundefs_in_val (Vconstr tau t vs)
-| Vfun_closed :
-    forall rho B f,
-      closed_fundefs B ->
-      closed_fundefs_in_fundefs B ->
-      (* fun_in_fundefs B (f, tau, xs, e) -> *)
-      (* Included _ (occurs_free e) (Union _ (FromList xs) (name_in_fundefs B)) -> *)
-      closed_fundefs_in_val (Vfun rho B f)
-| Vint_closed :
-    forall z, closed_fundefs_in_val (Vint z).
+      f' vs = Some v ->
+      closed_fundefs_in_val v.
 
-Definition closed_fundefs_in_env (S : Ensemble var) rho : Prop :=
-  lift_P_env S closed_fundefs_in_val rho.
-
-Lemma fun_in_fundefs_funs_in_fundef B B' f t xs e :
-  fun_in_fundefs B (f, t, xs, e) ->
-  funs_in_exp B' e ->
-  funs_in_fundef B' B.
-Proof.
-  induction B; intros Hin Hfuns.
-  - inv Hin.
-    + inv H. now eauto.
-    + constructor 2. eapply IHB; eauto.
-  - inv Hin.
-Qed.
-
-Axiom prims_closed_fundefs :
-  forall (f : prim) (f' : list val -> option val) vs v,
-    M.get f pr = Some f' ->
-    Forall closed_fundefs_in_val vs ->
-    f' vs = Some v ->
+  Lemma bstep_e_preserves_closed_fundefs rho e v c :
+    bstep_e pr cenv rho e v c ->
+    closed_fundefs_in_env (occurs_free e) rho ->
+    closed_fundefs_in_exp e ->
     closed_fundefs_in_val v.
-
-Lemma bstep_e_preserves_closed_fundefs rho e v c :
-  bstep_e pr rho e v c ->
-  closed_fundefs_in_env (occurs_free e) rho ->
-  closed_fundefs_in_exp e ->
-  closed_fundefs_in_val v.
-Proof.
-  intros Hstep Hcl1 Hcl2. induction Hstep.
-  - eapply IHHstep.
-    + subst. eapply lift_P_env_extend. 
-      * eapply lift_P_env_antimon; [| now eauto ].
-        rewrite occurs_free_Econstr.
-        eapply Included_Union_r.
-      * constructor. eapply lift_P_env_getlist; eauto.
-        rewrite occurs_free_Econstr. eapply Included_Union_l.
-    + intros B Hin. eauto.
-  - eapply IHHstep.
-    + subst. eapply lift_P_env_extend. 
-      * eapply lift_P_env_antimon; [| now eauto ].
-        rewrite occurs_free_Eproj.
-        eapply Included_Union_r.
-      * eapply Forall_nthN; [| eassumption ].
-        eapply lift_P_env_get in H; [| eassumption |].
-        now inv H. 
-        rewrite occurs_free_Eproj. eapply Included_Union_l.
-    + intros B Hin. eauto.
-  - eapply IHHstep.
-    + eapply lift_P_env_antimon; [| now eauto ].
-      eapply occurs_free_Ecase_Included.
-      eapply findtag_In_patterns. eassumption.
-    + intros B Hin. eapply Hcl2.
-      econstructor; eauto. apply findtag_In_patterns. eassumption.
-  - eapply IHHstep.
-    + eapply Hcl1 in H; [| now eauto ]. inv H.
-      apply find_def_correct in H1.  
-      eapply lift_P_env_antimon. eapply occurs_free_in_fun.
-      eassumption.
-      unfold closed_fundefs in H5. rewrite H5, Union_Empty_set_l.
-      eapply lift_P_env_setlist; [| | now eauto ].
-      * rewrite Setminus_Union_distr, Setminus_Empty_set, Union_Empty_set_r.
-        eapply  lift_P_env_def_funs.
-        rewrite Setminus_Included_Empty_set. now apply lift_P_env_Emtpy_set.
-        eapply Setminus_Included. now apply Included_refl.
-        intros f''. now constructor. 
-      * eapply lift_P_env_getlist; [ eassumption | | eassumption ].
-        rewrite occurs_free_Eapp. eapply Included_Union_l.
-    + intros B Hin.
-      eapply Hcl1 in H; [| now eauto ].
-      eapply find_def_correct in H1.
-      inv H. eapply H7. eapply fun_in_fundefs_funs_in_fundef; eassumption. 
-  - eapply IHHstep.
-    + eapply lift_P_env_def_funs.
-      * eapply lift_P_env_antimon; [| eassumption ].
-        rewrite occurs_free_Efun. eapply Included_Union_r.
-      * intros f. constructor. now eapply Hcl2.
-        intros B H. eapply Hcl2. now eauto.
-    + intros B Hin. eauto.
-  - eapply IHHstep.
-    + subst. eapply lift_P_env_extend. 
-      * eapply lift_P_env_antimon; [| now eauto ].
-        rewrite occurs_free_Eprim. eapply Included_Union_r.
-      * eapply prims_closed_fundefs; [ eassumption | | eassumption ].
-        eapply lift_P_env_getlist; [ eassumption | | eassumption ].
-        rewrite occurs_free_Eprim. eapply Included_Union_l.
-    + intros B Hin. eauto.
-Qed.
+  Proof.
+    intros Hstep Hcl1 Hcl2. induction Hstep.
+    - eapply IHHstep.
+      + subst. eapply lift_P_env_extend. 
+        * eapply lift_P_env_antimon; [| now eauto ].
+          rewrite occurs_free_Econstr.
+          eapply Included_Union_r.
+        * constructor. eapply lift_P_env_getlist; eauto.
+          rewrite occurs_free_Econstr. eapply Included_Union_l.
+      + intros B Hin. eauto.
+    - eapply IHHstep.
+      + subst. eapply lift_P_env_extend. 
+        * eapply lift_P_env_antimon; [| now eauto ].
+          rewrite occurs_free_Eproj.
+          eapply Included_Union_r.
+        * eapply Forall_nthN; [| eassumption ].
+          eapply lift_P_env_get in H; [| eassumption |].
+          now inv H. 
+          rewrite occurs_free_Eproj. eapply Included_Union_l.
+      + intros B Hin. eauto.
+    - eapply IHHstep.
+      + eapply lift_P_env_antimon; [| now eauto ].
+        eapply occurs_free_Ecase_Included.
+        eapply findtag_In_patterns. eassumption.
+      + intros B Hin. eapply Hcl2.
+        econstructor; eauto. apply findtag_In_patterns. eassumption.
+    - eapply IHHstep.
+      + eapply Hcl1 in H; [| now eauto ]. inv H.
+        apply find_def_correct in H1.  
+        eapply lift_P_env_antimon. eapply occurs_free_in_fun.
+        eassumption.
+        unfold closed_fundefs in H5. rewrite H5, Union_Empty_set_l.
+        eapply lift_P_env_setlist; [| | now eauto ].
+        * rewrite Setminus_Union_distr, Setminus_Empty_set, Union_Empty_set_r.
+          eapply  lift_P_env_def_funs.
+          rewrite Setminus_Included_Empty_set. now apply lift_P_env_Emtpy_set.
+          eapply Setminus_Included. now apply Included_refl.
+          intros f''. now constructor. 
+        * eapply lift_P_env_getlist; [ eassumption | | eassumption ].
+          rewrite occurs_free_Eapp. eapply Included_Union_l.
+      + intros B Hin.
+        eapply Hcl1 in H; [| now eauto ].
+        eapply find_def_correct in H1.
+        inv H. eapply H7. eapply fun_in_fundefs_funs_in_fundef; eassumption. 
+    - eapply IHHstep.
+      + eapply lift_P_env_def_funs.
+        * eapply lift_P_env_antimon; [| eassumption ].
+          rewrite occurs_free_Efun. eapply Included_Union_r.
+        * intros f. constructor. now eapply Hcl2.
+          intros B H. eapply Hcl2. now eauto.
+      + intros B Hin. eauto.
+    - eapply IHHstep.
+      + subst. eapply lift_P_env_extend. 
+        * eapply lift_P_env_antimon; [| now eauto ].
+          rewrite occurs_free_Eprim. eapply Included_Union_r.
+        * eapply prims_closed_fundefs; [ eassumption | | eassumption ].
+          eapply lift_P_env_getlist; [ eassumption | | eassumption ].
+          rewrite occurs_free_Eprim. eapply Included_Union_l.
+      + intros B Hin. eauto.
+  Qed.
 
 End Log_rel.
