theories/L6_PCPS/closure_conversion.v
@@ -12,461 +12,342 @@ Open Scope fun_scope.
 
 (** * Closure conversion as a relation  *)
 
-Inductive project_var :
-  Ensemble var -> (* Variables in the current scope *)
-  Ensemble var -> (* Names of the functions in the current function block *)
-  (var -> var) -> (* renaming of function names *)
-  var -> (* The environment argument *)
-  list var -> (* The environment *)
-  Ensemble var -> (* The free set *)
-  var -> (* Before projection *)
-  var -> (* After projection *)
-  exp_ctx -> (* Context that will perform the projection *)
-  Ensemble var -> (* The new free set *)
-  Prop :=
-| Var_in_Scope :
-    forall Scope Funs f Γ FVs S x,
-      In _ Scope x ->
-      project_var Scope Funs f Γ FVs S x x Hole_c S
-| Var_in_Funs :
-    forall Scope Funs f Γ FVs S x y t tau,
-      ~ In _ Scope x ->
-      In _ Funs x ->
-      In _ S y ->
-      project_var Scope Funs f Γ FVs S x y
-                  (Econstr_c y t tau [(f x); Γ] Hole_c) (Setminus _ S (Singleton _ y))
-| Var_in_FVs :
-    forall Scope Funs f Γ FVs S x y N tau,
-      ~ In _ Scope x ->
-      ~ In _ Funs x -> 
-      nthN FVs N = Some x ->
-      In _ S y ->
-      project_var Scope Funs f Γ FVs S x y
-                  (Eproj_c y tau N Γ Hole_c) (Setminus _ S (Singleton _ y)).
+Section CC.
+  Variable (clo_tag : cTag). (* Tag for closure records *)
 
-Inductive project_vars :
-  Ensemble var -> (* Variables in the current scope *)
-  Ensemble var -> (* Names of the functions in the current function block *)
-  (var -> var) -> (* renaming of function names *)
-  var -> (* The environment argument *)
-  list var -> (* The free variables *)
-  Ensemble var -> (* The free set *)
-  list var -> (* Before projection *)
-  list var -> (* After projection *)
-  exp_ctx -> (* Context that will perform the projection *)
-  Ensemble var -> (* The new free set *)
-  Prop :=
-| VarsNil :
-    forall Scope Funs f Γ FVs S,
-      project_vars Scope Funs f Γ FVs S [] [] Hole_c S
-| VarsCons :
-    forall Scope Funs f Γ FVs y y' ys ys' C1 C2 S1 S2 S3,
-      project_var Scope Funs f Γ FVs S1 y y' C1 S2 ->
-      project_vars Scope Funs f Γ FVs S2 ys ys' C2 S3 ->
-      project_vars Scope Funs f Γ FVs S1 (y :: ys) (y' :: ys') (comp_ctx_f C1 C2) S3.
+  Inductive project_var :
+    Ensemble var -> (* Variables in the current scope *)
+    Ensemble var -> (* Names of the functions in the current function block *)
+    (var -> var) -> (* renaming of function names *)
+    cTag -> (* tag of the current environment constructor *)
+    var -> (* The environment argument *)
+    list var -> (* The environment *)
+    Ensemble var -> (* The free set *)
+    var -> (* Before projection *)
+    var -> (* After projection *)
+    exp_ctx -> (* Context that will perform the projection *)
+    Ensemble var -> (* The new free set *)
+    Prop :=
+  | Var_in_Scope :
+      forall Scope Funs f c Γ FVs S x,
+        In _ Scope x ->
+        project_var Scope Funs f c Γ FVs S x x Hole_c S
+  | Var_in_Funs :
+      forall Scope Funs f c Γ FVs S x y,
+        ~ In _ Scope x ->
+        In _ Funs x ->
+        In _ S y ->
+        project_var Scope Funs f c Γ FVs S x y
+                    (Econstr_c y clo_tag [(f x); Γ] Hole_c) (Setminus _ S (Singleton _ y))
+  | Var_in_FVs :
+      forall Scope Funs f c Γ FVs S x y N,
+        ~ In _ Scope x ->
+        ~ In _ Funs x -> 
+        nthN FVs N = Some x ->
+        In _ S y ->
+        project_var Scope Funs f c Γ FVs S x y
+                    (Eproj_c y c N Γ Hole_c) (Setminus _ S (Singleton _ y)).
 
-Inductive make_closures :
-  fundefs -> (* The function block *)
-  Ensemble var -> (* The free set *)
-  var -> (* The environment variable *)
-  exp_ctx -> (* The context that constructs the closures *)
-  (var -> var) -> (* The renaming *)
-  Ensemble var -> (* The new free set *)
-  Prop :=
-| closures_Fnil :
-    forall Γ f S,
-      make_closures Fnil S Γ Hole_c f S
-| closures_Fcons :
-    forall f f' xs tau e B Γ C tau' t' g g' S S',
-      make_closures B (Setminus _ S (Singleton _ f')) Γ C g S' ->
-      In _ S f' ->
-      f_eq (g {f ~> f'}) g' ->
-      make_closures (Fcons f tau xs e B) S Γ
-                    (Econstr_c f tau' t' [f' ; Γ] C)
-                    g' S'.
+  Inductive project_vars :
+    Ensemble var -> (* Variables in the current scope *)
+    Ensemble var -> (* Names of the functions in the current function block *)
+    (var -> var) -> (* renaming of function names *)
+    cTag -> (* tag of the current environment constructor *)
+    var -> (* The environment argument *)
+    list var -> (* The free variables *)
+    Ensemble var -> (* The free set *)
+    list var -> (* Before projection *)
+    list var -> (* After projection *)
+    exp_ctx -> (* Context that will perform the projection *)
+    Ensemble var -> (* The new free set *)
+    Prop :=
+  | VarsNil :
+      forall Scope Funs f c Γ FVs S,
+        project_vars Scope Funs f c Γ FVs S [] [] Hole_c S
+  | VarsCons :
+      forall Scope Funs f c Γ FVs y y' ys ys' C1 C2 S1 S2 S3,
+        project_var Scope Funs f c Γ FVs S1 y y' C1 S2 ->
+        project_vars Scope Funs f c Γ FVs S2 ys ys' C2 S3 ->
+        project_vars Scope Funs f c Γ FVs S1 (y :: ys) (y' :: ys') (comp_ctx_f C1 C2) S3.
 
-Inductive Closure_conversion :
-  Ensemble var -> (* Variables in the current scope *)
-  Ensemble var -> (* Names of the functions in the current function block *)
-  (var -> var) -> (* renaming of function names *)
-  var -> (* The environment argument *)
-  list var -> (* The free variables - needs to be ordered *)
-  exp -> (* Before cc *)
-  exp -> (* After cc *)
-  exp_ctx -> (* The context that the output expression should be put in *)
-  Prop :=
-| CC_Econstr :
-    forall Scope Funs f Γ FVs S' S x ys ys' C C' tau tau' t e e',
-      (* Variables for projected vars should not shadow the variables in
+  Inductive make_closures :
+    fundefs -> (* The function block *)
+    Ensemble var -> (* The free set *)
+    var -> (* The environment variable *)
+    exp_ctx -> (* The context that constructs the closures *)
+    (var -> var) -> (* The renaming *)
+    Ensemble var -> (* The new free set *)
+    Prop :=
+  | closures_Fnil :
+      forall Γ f S,
+        make_closures Fnil S Γ Hole_c f S
+  | closures_Fcons :
+      forall f f' xs t e B Γ C g g' S S',
+        make_closures B (Setminus _ S (Singleton _ f')) Γ C g S' ->
+        In _ S f' ->
+        f_eq (g {f ~> f'}) g' ->
+        make_closures (Fcons f t xs e B) S Γ
+                      (Econstr_c f clo_tag [f' ; Γ] C)
+                      g' S'.
+
+  Inductive Closure_conversion :
+    Ensemble var -> (* Variables in the current scope *)
+    Ensemble var -> (* Names of the functions in the current function block *)
+    (var -> var) -> (* renaming of function names *)
+    cTag -> (* tag of the current environment constructor *)
+    var -> (* The environment argument *)
+    list var -> (* The free variables - needs to be ordered *)
+    exp -> (* Before cc *)
+    exp -> (* After cc *)
+    exp_ctx -> (* The context that the output expression should be put in *)
+    Prop :=
+  | CC_Econstr :
+      forall Scope Funs f c Γ FVs S' S x ys ys' C C' t e e',
+        (* Variables for projected vars should not shadow the variables in
          scope, i.e. Scope U FV U { Γ } *)
-      Disjoint _ S (Union _ Scope
-                          (Union _ (image f (Setminus _ Funs Scope))
-                                 (Union _ (FromList FVs) (Singleton _ Γ)))) ->
-      project_vars Scope Funs f Γ FVs S ys ys' C S' ->
-      (* We do not care about ys'. Should never be accessed again so do not
+        Disjoint _ S (Union _ Scope
+                            (Union _ (image f (Setminus _ Funs Scope))
+                                   (Union _ (FromList FVs) (Singleton _ Γ)))) ->
+        project_vars Scope Funs f c Γ FVs S ys ys' C S' ->
+        (* We do not care about ys'. Should never be accessed again so do not
          add them aτ the current scope *)
-      Closure_conversion (Union _ (Singleton _ x) Scope) Funs f Γ FVs e e' C' ->
-      Closure_conversion Scope Funs f Γ FVs (Econstr x tau t ys e)
-                         (Econstr x tau' t ys' (C' |[ e' ]|)) C
-| CC_Ecase :
-    forall Scope Funs f Γ FVs x x' C S S' pats pats',
-      Disjoint _ S (Union _ Scope
-                          (Union _ (image f (Setminus _ Funs Scope))
-                                 (Union _ (FromList FVs) (Singleton _ Γ)))) ->
-      project_var Scope Funs f Γ FVs S x x' C S' ->
-      Forall2 (fun (pat pat' : tag * exp) =>
-                 (fst pat) = (fst pat') /\
-                 exists C' e',
-                   snd pat' = C' |[ e' ]| /\
-                   Closure_conversion Scope Funs f Γ FVs (snd pat) e' C')
-              pats pats' ->
-      Closure_conversion Scope Funs f Γ FVs (Ecase x pats) (Ecase x' pats') C
-| CC_Eproj :
-    forall Scope Funs f Γ FVs S S' x y y' C C' tau tau' N e e',
-      Disjoint _ S (Union _ Scope
-                          (Union _ (image f (Setminus _ Funs Scope))
-                                 (Union _ (FromList FVs) (Singleton _ Γ)))) ->
-      project_var Scope Funs f Γ FVs S y y' C S' ->
-      Closure_conversion (Union _ (Singleton _ x) Scope) Funs f Γ FVs e e' C' ->
-      Closure_conversion Scope Funs f Γ FVs (Eproj x tau N y e)
-                         (Eproj x tau' N y' (C' |[ e' ]|)) C
-| CC_Efun :
-    forall Scope Funs f f' Γ Γ' FVs FVs' FVs'' B B' e e' C C' Ce S1 S1' S2 S2' S3 tau t,
-      (* The environment contains all the variables that are free in B *)
-      Same_set _ (occurs_free_fundefs B) (FromList FVs') ->
-      (* Project the FVs to construct the environment *)
-      Disjoint _ S1 (Union _ Scope
-                          (Union _ (image f (Setminus _ Funs Scope))
-                                 (Union _ (FromList FVs) (Singleton _ Γ)))) ->
-      project_vars Scope Funs f Γ FVs S1 FVs' FVs'' C' S1' ->
-      (* Γ' is the variable that will hold the record of the environment *)
-      Disjoint _ S3 (Union _ (name_in_fundefs B)
-                           (Union _ Scope
-                                  (Union _ (image f (Setminus _ Funs Scope))
-                                         (Union _ (FromList FVs) (Singleton _ Γ))))) ->
-      In _ S3 Γ' ->
-      Disjoint _ S2 (Union _ (bound_var_fundefs B)
-                           (Union _ (Singleton _ Γ')
-                                  (Union _ Scope
-                                         (Union _ (image f (Setminus _ Funs Scope))
-                                                (Union _ (FromList FVs) (Singleton _ Γ)))))) ->
-      make_closures B S2  Γ' C f' S2' ->
-      Closure_conversion_fundefs (name_in_fundefs B) f' FVs' B B' ->
-      Closure_conversion (Union _ (name_in_fundefs B) Scope) Funs f Γ FVs e e' Ce  ->
-      Closure_conversion Scope Funs f Γ FVs (Efun B e)
-                         (Efun B' (C |[ Ce |[ e' ]| ]|)) (comp_ctx_f C' (Econstr_c Γ' tau t FVs'' Hole_c))
-| CC_Eapp :
-    forall Scope Funs g Γ FVs f f' f'' env' ys ys' C S S' tau tau',
-      Disjoint _ S (Union _ Scope
-                          (Union _ (image g (Setminus _ Funs Scope))
-                                 (Union _ (FromList FVs) (Singleton _ Γ)))) ->
-      (* Project the function name and the actual parameter *)
-      project_vars Scope Funs g Γ FVs S (f :: ys) (f' :: ys') C S' ->
-      (* (* Project the actual parameters *) *)
-      (* project_vars Scope Funs Γ FVs S1 ys ys' C2 S2 -> *)
-      (* The name of the function pointer and the name of the environment
+        Closure_conversion (Union _ (Singleton _ x) Scope) Funs f c Γ FVs e e' C' ->
+        Closure_conversion Scope Funs f c Γ FVs (Econstr x t ys e)
+                           (Econstr x t ys' (C' |[ e' ]|)) C
+  | CC_Ecase :
+      forall Scope Funs f c Γ FVs x x' C S S' pats pats',
+        Disjoint _ S (Union _ Scope
+                            (Union _ (image f (Setminus _ Funs Scope))
+                                   (Union _ (FromList FVs) (Singleton _ Γ)))) ->
+        project_var Scope Funs f c Γ FVs S x x' C S' ->
+        Forall2 (fun (pat pat' : cTag * exp) =>
+                   (fst pat) = (fst pat') /\
+                   exists C' e',
+                     snd pat' = C' |[ e' ]| /\
+                                            Closure_conversion Scope Funs f c Γ FVs (snd pat) e' C')
+                pats pats' ->
+        Closure_conversion Scope Funs f c Γ FVs (Ecase x pats) (Ecase x' pats') C
+  | CC_Eproj :
+      forall Scope Funs f c Γ FVs S S' x y y' C C' t N e e',
+        Disjoint _ S (Union _ Scope
+                            (Union _ (image f (Setminus _ Funs Scope))
+                                   (Union _ (FromList FVs) (Singleton _ Γ)))) ->
+        project_var Scope Funs f c Γ FVs S y y' C S' ->
+        Closure_conversion (Union _ (Singleton _ x) Scope) Funs f c Γ FVs e e' C' ->
+        Closure_conversion Scope Funs f c Γ FVs (Eproj x t N y e)
+                           (Eproj x t N y' (C' |[ e' ]|)) C
+  | CC_Efun :
+      forall Scope Funs f f' c Γ c' Γ' FVs FVs' FVs'' B B' e e' C C' Ce S1 S1' S2 S2' S3,
+        (* The environment contains all the variables that are free in B *)
+        Same_set _ (occurs_free_fundefs B) (FromList FVs') ->
+        (* Project the FVs to construct the environment *)
+        Disjoint _ S1 (Union _ Scope
+                             (Union _ (image f (Setminus _ Funs Scope))
+                                    (Union _ (FromList FVs) (Singleton _ Γ)))) ->
+        project_vars Scope Funs f c Γ FVs S1 FVs' FVs'' C' S1' ->
+        (* Γ' is the variable that will hold the record of the environment *)
+        Disjoint _ S3 (Union _ (name_in_fundefs B)
+                             (Union _ Scope
+                                    (Union _ (image f (Setminus _ Funs Scope))
+                                           (Union _ (FromList FVs) (Singleton _ Γ))))) ->
+        In _ S3 Γ' ->
+        Disjoint _ S2 (Union _ (bound_var_fundefs B)
+                             (Union _ (Singleton _ Γ')
+                                    (Union _ Scope
+                                           (Union _ (image f (Setminus _ Funs Scope))
+                                                  (Union _ (FromList FVs) (Singleton _ Γ)))))) ->
+        make_closures B S2  Γ' C f' S2' ->
+        Closure_conversion_fundefs (name_in_fundefs B) f' c' FVs' B B' ->
+        Closure_conversion (Union _ (name_in_fundefs B) Scope) Funs f c Γ FVs e e' Ce  ->
+        Closure_conversion Scope Funs f c Γ FVs (Efun B e)
+                           (Efun B' (C |[ Ce |[ e' ]| ]|)) (comp_ctx_f C' (Econstr_c Γ' c' FVs'' Hole_c))
+  | CC_Eapp :
+      forall Scope Funs g c Γ FVs f f' f'' ft env' ys ys' C S S',
+        Disjoint _ S (Union _ Scope
+                            (Union _ (image g (Setminus _ Funs Scope))
+                                   (Union _ (FromList FVs) (Singleton _ Γ)))) ->
+        (* Project the function name and the actual parameter *)
+        project_vars Scope Funs g c Γ FVs S (f :: ys) (f' :: ys') C S' ->
+        (* (* Project the actual parameters *) *)
+        (* project_vars Scope Funs Γ FVs S1 ys ys' C2 S2 -> *)
+        (* The name of the function pointer and the name of the environment
          should not shadow the variables in the current scope and the
          variables that where used in the projections *)
-      In _ S' f'' -> In _ S' env' -> f'' <> env' ->
-      Closure_conversion Scope Funs g Γ FVs (Eapp f ys)
-                         (Eproj f'' tau 0%N f'
-                                (Eproj env' tau' 1%N f'
-                                       (Eapp f'' (env' :: ys')))) C
-| CC_Eprim :
-    forall Scope Funs g Γ FVs S S' x ys ys' C C' tau tau' f e e',
-      Disjoint _ S (Union _ Scope
-                          (Union _ (image g (Setminus _ Funs Scope))
-                                 (Union _ (FromList FVs) (Singleton _ Γ)))) ->
-      project_vars Scope Funs g Γ FVs S ys ys' C S' ->
-      Closure_conversion (Union _ (Singleton _ x) Scope) Funs g Γ FVs e e' C' ->
-      Closure_conversion Scope Funs g Γ FVs (Eprim x tau f ys e)
-                         (Eprim x tau' f ys' (C' |[ e' ]|)) C
-with Closure_conversion_fundefs :
-  Ensemble var -> (* The function names in the current block *)
-  (var -> var) -> (* renaming of function names *)
-  list var -> (* The environment *)
-  fundefs -> (* Before cc *)
-  fundefs -> (* After cc *)
-  Prop :=
-| CC_Fcons :
-    forall Funs g Γ' FVs S f tau tau' ys e e' C defs defs',
-      (* The environment binding should not shadow the current scope
+        In _ S' f'' -> In _ S' env' -> f'' <> env' ->
+        Closure_conversion Scope Funs g c Γ FVs (Eapp f ft ys)
+                           (Eproj f'' clo_tag 0%N f'
+                                  (Eproj env' clo_tag 1%N f'
+                                         (Eapp f'' ft (env' :: ys')))) C
+  | CC_Eprim :
+      forall Scope Funs g c Γ FVs S S' x ys ys' C C' f e e',
+        Disjoint _ S (Union _ Scope
+                            (Union _ (image g (Setminus _ Funs Scope))
+                                   (Union _ (FromList FVs) (Singleton _ Γ)))) ->
+        project_vars Scope Funs g c Γ FVs S ys ys' C S' ->
+        Closure_conversion (Union _ (Singleton _ x) Scope) Funs g c Γ FVs e e' C' ->
+        Closure_conversion Scope Funs g c Γ FVs (Eprim x f ys e)
+                           (Eprim x f ys' (C' |[ e' ]|)) C
+  with Closure_conversion_fundefs :
+         Ensemble var -> (* The function names in the current block *)
+         (var -> var) -> (* renaming of function names *)
+         cTag -> (* tag of the current environment constructor *)
+         list var -> (* The environment *)
+         fundefs -> (* Before cc *)
+         fundefs -> (* After cc *)
+         Prop :=
+       | CC_Fcons :
+           forall Funs g c Γ' FVs S f t ys e e' C defs defs',
+             (* The environment binding should not shadow the current scope
          (i.e. the names of the mut. rec. functions and the other arguments) *)
-      Disjoint _ S (Union _ (image g Funs) (Union _ (FromList ys) (bound_var e))) ->
-      In _ S  Γ' ->
-      Closure_conversion_fundefs Funs g FVs defs defs' ->
-      Closure_conversion (FromList ys) Funs g Γ' FVs e e' C ->
-      Closure_conversion_fundefs Funs g FVs (Fcons f tau ys e defs )
-                                 (Fcons (g f) tau' (Γ' :: ys) (C |[ e' ]|) defs')
-| CC_Fnil :
-    forall Funs g FVs,
-      Closure_conversion_fundefs Funs g FVs Fnil Fnil.
+             Disjoint _ S (Union _ (image g Funs) (Union _ (FromList ys) (bound_var e))) ->
+             In _ S  Γ' ->
+             Closure_conversion_fundefs Funs g c FVs defs defs' ->
+             Closure_conversion (FromList ys) Funs g c Γ' FVs e e' C ->
+             Closure_conversion_fundefs Funs g c FVs (Fcons f t ys e defs )
+                                        (Fcons (g f) t (Γ' :: ys) (C |[ e' ]|) defs')
+       | CC_Fnil :
+           forall Funs g c FVs,
+             Closure_conversion_fundefs Funs g c FVs Fnil Fnil.
 
 
-(* Definition Closure_conversion_alpha (Scope Funs : Ensemble var) (Γ : var) *)
-(*            (FVs : list var) (C : exp_ctx) sbst *)
-(* : relation exp  := *)
-(*   fun e e' => *)
-(*     exists e'' C'', Closure_conversion Scope Funs Γ FVs e e'' C'' /\ *)
-(*                Alpha_conv_ctx C'' C sbst /\ Alpha_conv e'' e' sbst. *)
+  (** * Computational defintion of closure conversion *)
 
-(* Definition Closure_conversion_fundefs_alpha (Funs : Ensemble var) (FVs : list var) sbst *)
-(* : relation fundefs  := *)
-(*   relations.compose (Closure_conversion_fundefs Funs FVs) (fun B B' => Alpha_conv_fundefs B B' sbst). *)
+  Inductive VarInfo : Type :=
+  (* A free variable, i.e. a variable outside the scope of the current function.
+   The argument is position of a free variable in the env record *)
+  | FVar : N -> VarInfo
+  (* A function defined in the current block of function definitions. The first
+   argument is the new name of the function (code pointer) *)
+  | MRFun : var -> VarInfo
+  (* A variable declared in the scope of the current function *)
+  | BoundVar : VarInfo.
 
+  (* Maps variables to [VarInfo] *)
+  Definition VarInfoMap := Maps.PTree.t VarInfo.
 
-(** * Computational defintion of closure conversion *)
-
-Record FunInfo : Type :=
-  mkFunInfo
-    { (* free variables of the function definition block *)
-      fv_set_def : FVSet;
-      (* the names of the functions in the block *)
-      rec_names  : FVSet }.
-
-(** Maps function name to [FunInfo] *)
-Definition FunInfoMap := Maps.PTree.t FunInfo.
-
-Definition TypeMap := Maps.PTree.t type.
-
-Inductive VarInfo : Type :=
-(* A free variable, i.e. a variable outside the scope of the current function.
-   The first argument is position of a free variable in the env record and the
-   second its type *)
-| FVar : N -> type -> VarInfo
-(* A function defined in the current block of function definitions. The first
-   argument is the new name of the function (code pointer), the second its the
-   type of the function and the third the type of the
-   closure *)
-| MRFun : var -> type -> type -> VarInfo
-(* A variable declared in the scope of the current function *)
-| BoundVar : type -> VarInfo.
-
-(* Maps variables to [VarInfo] *)
-Definition VarInfoMap := Maps.PTree.t VarInfo.
-
-(** The state is the next available free variable and the type dictionary *)
-Definition ccstate := state (var * TDict.t).
-
-(** Get a fresh name *)
-Definition get_name : ccstate var :=
-  p <- get ;;
-  let '(n, d) := p in
-  put ((n+1)%positive, d) ;;
-  ret n.
-
-(** Setter and getter for types *)
-Definition set_typeinfo (t : typeinfo) : ccstate type :=
-  p <- get ;;
-  let '(n, d) := p in
-  let (h, d') := TDict.hash t d in
-  put (n, d') ;;
-  ret h.
-
-Definition get_typeinfo (i : type) : ccstate typeinfo :=
-  p <- get ;;
-  let '(n, d) := p in
-  match TDict.get i d with
-    | Some typinfo => ret typinfo
-    | None => ret Tunknown (* should not happen *)
-  end.
-
-(** Construct the [FunInfo] map *)
-Fixpoint exp_info (e : exp) (acc : FunInfoMap) : FunInfoMap :=
-  match e with
-    | Econstr x tau c ys e =>
-      exp_info e acc
-    | Ecase x pats =>
-      fold_left (fun map te => exp_info (snd te) map) pats acc 
-    | Eproj x tau n y e =>
-      exp_info e acc
-    | Efun defs e =>
-      let names := fundefs_names defs in
-      let acc' := fundefs_info defs (fundefs_fv defs names) names acc in
-      exp_info e acc'
-    | Eapp x xs => acc
-    | Eprim x tau prim ys e =>
-      exp_info e acc
-  end
-with fundefs_info (defs : fundefs) (fv : FVSet) (names : FVSet)
-                  (acc : FunInfoMap) : FunInfoMap :=
-       match defs with
-         | Fcons f tau ys e defs' =>
-           let acc' := Maps.PTree.set f
-                                      {| fv_set_def := fv;
-                                         rec_names := names |}
-                                      acc in
-           let acc'' := exp_info e acc' in
-           fundefs_info defs' names fv acc'' 
-         | Fnil => acc
-       end.
-
-Section CC.
-  Context (utag : tag) (* Tag for types with unique constructor *)
-          (env_tag : tag) (* Tag for the type of environments *)
-          (tag_bij : tag -> tag) (* mapping from function tags to closure 
-                                    records tags *)
-          (unknown_type : type).
+  Record state_contents :=
+    mkCont { next_var : var ; nect_cTag : cTag ; next_iTag : iTag; cenv : cEnv }.
+  
+  (** The state is the next available free variable, cTag and iTag and the tag environment *)
+  Definition ccstate :=
+    state state_contents.
+  
+  (** Get a fresh name *)
+  Definition get_name : ccstate var :=
+    p <- get ;;
+    let '(mkCont n c i e) := p in
+    put (mkCont ((n+1)%positive) c i e) ;;
+    ret n.
+  
+  Definition make_record_cTag (n : N) : ccstate cTag :=
+    p <- get ;;
+    let '(mkCont x c i e) := p  in
+    let inf := (i, n, 0%N) : cTyInfo in
+    let e' := ((M.set c inf e) : cEnv) in
+    put (mkCont x (c+1)%positive (i+1)%positive e') ;;
+    ret c.
 
   (** Looks up a variable in the map and handles it appropriately *) 
-  Definition get_var (x : var) (map : VarInfoMap) (Γ : var)
-  : ccstate (var * type * (exp -> exp)) :=
+  Definition get_var (x : var) (map : VarInfoMap) (c : cTag) (Γ : var)
+  : ccstate (var * (exp -> exp)) :=
     match Maps.PTree.get x map with
       | Some entry =>
         match entry with
-          | FVar pos typ =>
+          | FVar pos =>
             (* pick a fresh name *)
             y <- get_name ;;
-            ret (y, typ, fun e => Eproj y typ pos Γ e)   
-          | MRFun code_ptr typ cl_typ =>
+            ret (y, fun e => Eproj y c pos Γ e)   
+          | MRFun code_ptr  =>
             (* get the new name of the function and pack it together with the
                current environment argument to construct the closure *)
             y <- get_name ;;
-            ret (y, cl_typ, fun e => Econstr y cl_typ utag [code_ptr; Γ] e)
-          | BoundVar typ => ret (x, typ, id)
+            ret (y, fun e => Econstr y clo_tag [code_ptr; Γ] e)
+          | BoundVar => ret (x, id)
         end
-      | None => ret (x, 1%positive, id) (* should never reach here *)
+      | None => ret (x, id) (* should never reach here *)
     end.
-
+  
   Fixpoint get_vars (xs : list var) (map : VarInfoMap)
-           (cl : var) : ccstate (list var * (exp -> exp)) :=
+           (c : cTag) (Γ : var) : ccstate (list var * (exp -> exp)) :=
     match xs with
       | [] => ret ([], id)
       | x :: xs =>
-        t1 <- get_var x map cl ;;
+        t1 <- get_var x map c Γ ;;
         let '(y, f) := t1 in
-        t2 <- get_vars xs map cl ;; 
+        t2 <- get_vars xs map c Γ ;; 
         let '(ys, f') := t2 in
-        ret (fst y :: ys, fun e => f (f' e))
-    end.
-
-  Fixpoint get_vars_with_types (xs : list var) (map : VarInfoMap) (cl : var)
-  : ccstate (list var * list type * (exp -> exp)) :=
-    match xs with
-      | [] => ret ([], [], id)
-      | x :: xs =>
-        t1 <- get_var x map cl ;;
-        let '(y, f) := t1 in
-        t2 <- get_vars_with_types xs map cl ;; 
-        let '(ys, ts, f') := t2 in
-        ret (fst y :: ys, snd y :: ts, fun e => f (f' e))
+        ret (y :: ys, fun e => f (f' e))
     end.
 
   (** Construct the closure environment and the new variable map *)
   Definition make_env (fv : FVSet) (mapfv_new : VarInfoMap)
-             (mapfv_old : VarInfoMap) (Γ_new Γ_old : var)
-  : ccstate (type * VarInfoMap * (exp -> exp)) :=
+             (mapfv_old : VarInfoMap) (c_old : cTag) (Γ_new Γ_old : var)
+  : ccstate (cTag * VarInfoMap * (exp -> exp)) :=
     (* put the free variables in a new map *)
     let fvs := PS.elements fv in
-    let map_new' :=
+    let '(map_new', n) :=
         (fix add_fvs l n map :=
            match l with
-             | [] => map
+             | [] => (map, n)
              | x :: xs =>
-               let typ :=
-                   match Maps.PTree.get x mapfv_old with
-                     | Some entry  =>
-                       match entry with
-                         | FVar _ t | BoundVar t
-                         | MRFun _ _ t => t
-                       end
-                     | None => 1%positive (* should not happen *)
-                   end
-               in
-               add_fvs xs (n + 1)%N (Maps.PTree.set x (FVar n typ) map)
+               add_fvs xs (n + 1)%N (Maps.PTree.set x (FVar n) map)
            end) fvs 0%N (Maps.PTree.empty VarInfo)
     in
-    t1 <- get_vars_with_types fvs mapfv_old Γ_old ;;
-    let '(fv', ts, g') :=  t1 in
-    env_typ <- set_typeinfo (Tdata [(env_tag, ts)]) ;;
-    ret (env_typ, map_new',
-         fun e => g' (Econstr Γ_new env_typ utag fv' e)).
-
-(* recursive lookup for types -- needs termination proof *)
-(* Fixpoint closure_type (fun_typ env_type : type) : ccstate type := *)
-(*   ftyp <- get_typeinfo fun_typ ;; *)
-(*   match ftyp with *)
-(*     | Tfun tag lst => *)
-(*       lst' <- mapM (fun f => closure_type f env_type) lst ;; *)
-(*       let ptr_inf := Tfun tag (env_type :: lst') in *)
-(*       ptr_typ <- set_typeinfo ptr_inf ;;  *)
-(*       let clo_inf := Tdata [(tag_bij tag, [ptr_typ; env_type])] in *)
-(*       typ <- set_typeinfo clo_inf ;; *)
-(*       ret typ *)
-(*     | _ => ret fun_typ *)
-(*   end. *)
+    t1 <- get_vars fvs mapfv_old c_old Γ_old ;;
+    let '(fv', g') :=  t1 in
+    c_new <- make_record_cTag n ;;
+    ret (c_new, map_new', fun e => g' (Econstr Γ_new c_new fv' e)).
   
   (** Construct closures after a function definition block *)
   Fixpoint make_full_closure (defs : fundefs) (mapfv_new mapfv_old : VarInfoMap)
-           (Γ : var) (env_type : type)
+           (Γ : var)
   : ccstate (VarInfoMap * VarInfoMap * (exp -> exp)) :=
     match defs with
       | Fcons f typ xs e defs' =>
         (* The new name of the function *)
         code_ptr <- get_name ;;
-        t <- make_full_closure defs' mapfv_new mapfv_old Γ env_type ;;
+        t <- make_full_closure defs' mapfv_new mapfv_old Γ ;;
         let '(mapfv_new', mapfv_old', g') := t in
-        tinf <- get_typeinfo typ ;;
-        p <- match tinf with
-               | Tfun tag args =>
-                 (* The new type of the code pointer *)
-                 (* XXX change args type - This is wrong *)
-                 let tinf' := Tfun tag (env_type :: args) in
-                 typ' <- set_typeinfo tinf' ;;
-                 (* The type of the closure *)
-                 let tinf'' := Tdata [(tag_bij tag, [typ'; unknown_type])] in
-                 typ'' <- set_typeinfo tinf'' ;;
-                  ret (typ', typ'') 
-               | _ => ret (1%positive, 1%positive)
-             end ;;
-        let (typ', typ'') := p in (* (type of code ptr * type of closure) *)
         (* update the new map *)
         let mapfv_new'' :=
-            Maps.PTree.set f (MRFun code_ptr typ' typ'') mapfv_new'
+            Maps.PTree.set f (MRFun code_ptr) mapfv_new'
         in
         (* update the old map *)
         let mapfv_old'' :=
-            Maps.PTree.set f (BoundVar typ'') mapfv_old'
+            Maps.PTree.set f BoundVar mapfv_old'
         in
         ret (mapfv_new'', mapfv_old'',
-             (fun e => Econstr f typ'' utag [code_ptr; Γ] (g' e)))
+             (fun e => Econstr f clo_tag [code_ptr; Γ] (g' e)))
       | Fnil => ret (mapfv_new, mapfv_old, id)
     end.
 
   (** Add some bound variables in the map *)
-  Fixpoint add_params args args_typ (mapfv : VarInfoMap) : VarInfoMap :=
+  Fixpoint add_params args  (mapfv : VarInfoMap) : VarInfoMap :=
     match args with
       | [] => mapfv
       | x :: xs =>
-        let (typ, typs) :=
-            match args_typ with
-              | [] => (1%positive, [])
-              | t :: ts => (t, ts) 
-            end
-        in
-        M.set x (BoundVar typ) (add_params xs typs mapfv)
+        M.set x BoundVar (add_params xs mapfv)
     end.
-  
-  (* Todo : Fix argument type bug *)
+
   Fixpoint exp_closure_conv (e : exp) (mapfv : VarInfoMap)
-           (Γ : var) : ccstate (exp * (exp -> exp)) := 
+           (c : cTag) (Γ : var) : ccstate (exp * (exp -> exp)) := 
     match e with
-      | Econstr x typ c ys e' =>
-        t1 <- get_vars ys mapfv Γ ;;
+      | Econstr x tag ys e' =>
+        t1 <- get_vars ys mapfv c Γ ;;
         let '(ys', f) := t1 in
-        ef <- exp_closure_conv e' (Maps.PTree.set x (BoundVar typ) mapfv) Γ ;;
-        ret (Econstr x typ c ys' ((snd ef) (fst ef)), f)
+        ef <- exp_closure_conv e' (Maps.PTree.set x BoundVar mapfv) c Γ ;;
+        ret (Econstr x tag ys' ((snd ef) (fst ef)), f)
       | Ecase x pats =>
         pats' <-
         (fix mapM_cc l :=
          match l with
            | [] => ret []
            | (y, e) :: xs =>
-             ef <- exp_closure_conv e mapfv Γ ;;
+             ef <- exp_closure_conv e mapfv c Γ ;;
              xs' <- mapM_cc xs ;;
              ret ((y, ((snd ef) (fst ef))) :: xs')
          end) pats;;
-        t1 <- get_var x mapfv Γ ;;
+        t1 <- get_var x mapfv c Γ ;;
         (* let pats_st := List.map (fun (p : tag * exp) => *)
         (*                           let (t, e) := p in *)
         (*                           e' <- exp_closure_conv e mapfv Γ ;; *)
@@ -478,121 +359,103 @@ Section CC.
         (*                 let e_st := exp_closure_conv e mapfv Γ in *)
         (*                 e' <-  e_st ;; *)
         (*                 ret (t, e')) pats ;; *)
-        let '(x', _, f1) := t1 in           
+        let '(x', f1) := t1 in           
         ret (Ecase x' pats', f1)
-      | Eproj x typ n y e' =>
-        t1 <- get_var y mapfv
-           Γ ;;
-        let '(y', _, f) := t1 in
-        ef <- exp_closure_conv e' (Maps.PTree.set x (BoundVar typ) mapfv) Γ ;;
-        ret (Eproj x typ n y' ((snd ef) (fst ef)), f)
+      | Eproj x tag n y e' =>
+        t1 <- get_var y mapfv c Γ ;;
+        let '(y', f) := t1 in
+        ef <- exp_closure_conv e' (Maps.PTree.set x BoundVar mapfv) c Γ ;;
+        ret (Eproj x tag n y' ((snd ef) (fst ef)), f)
       | Efun defs e =>
         let names := fundefs_names defs in
         let fv := fundefs_fv defs names in
         Γ' <- get_name ;;
-        t1 <- make_env fv (Maps.PTree.empty VarInfo) mapfv Γ' Γ ;;
-        let '(env_type, mapfv_new, g1) := t1 in
-        t2 <- make_full_closure defs mapfv_new mapfv Γ' env_type ;;
+        t1 <- make_env fv (Maps.PTree.empty VarInfo) mapfv c Γ' Γ ;;
+        let '(c', mapfv_new, g1) := t1 in
+        t2 <- make_full_closure defs mapfv_new mapfv Γ'  ;;
         let '(mapfv_new', mapfv_old', g2) := t2 in
-        ef <- exp_closure_conv e mapfv_old' Γ ;;
-        defs' <- fundefs_closure_conv defs mapfv_new' ;;
+        ef <- exp_closure_conv e mapfv_old' c Γ ;;
+        defs' <- fundefs_closure_conv defs mapfv_new' c' ;;
         ret (Efun defs' (g2 ((snd ef) (fst ef))), g1)
-      | Eapp f xs =>
-        t1 <- get_var f mapfv Γ ;;
-        let '(f', typ, g1) := t1 in     
-        t2 <- get_vars xs mapfv Γ ;;
+      | Eapp f ft xs =>
+        t1 <- get_var f mapfv c Γ ;;
+        let '(f', g1) := t1 in     
+        t2 <- get_vars xs mapfv c Γ ;;
         let '(xs', g2) := t2 in
         ptr <- get_name ;;
         Γ <- get_name ;;
-        typinf <- get_typeinfo typ;;    
-        let ftyp :=
-            match typinf with
-              | Tdata [(_, (ftyp :: _))] => ftyp
-              | _ => 1%positive (* should not happen *) 
-            end
-        in
-        ret (Eproj ptr ftyp 0 f'
-                   (Eproj Γ unknown_type 1 f'
-                          (Eapp ptr (Γ :: xs'))), fun e => g1 (g2 e))
-    | Eprim x typ prim ys e' =>
-      t1 <- get_vars ys mapfv Γ ;;
+        ret (Eproj ptr clo_tag 0 f'
+                   (Eproj Γ clo_tag 1 f'
+                          (Eapp ptr ft (Γ :: xs'))), fun e => g1 (g2 e))
+    | Eprim x prim ys e' =>
+      t1 <- get_vars ys mapfv c Γ ;;
       let '(ys', f) := t1 in
-      ef <- exp_closure_conv e' (Maps.PTree.set x (BoundVar typ) mapfv) Γ ;;
-      ret (Eprim x typ prim ys' ((snd ef) (fst ef)), f)
+      ef <- exp_closure_conv e' (Maps.PTree.set x BoundVar mapfv) c Γ ;;
+      ret (Eprim x prim ys' ((snd ef) (fst ef)), f)
     end
-  with fundefs_closure_conv (defs : fundefs) (mapfv : VarInfoMap)
+  with fundefs_closure_conv (defs : fundefs) (mapfv : VarInfoMap) (c : cTag)
        : ccstate fundefs  :=
          match defs with
-           | Fcons f typ ys e defs' =>
-             typinf <- get_typeinfo typ ;;
-             let args_typ :=
-                 match typinf with
-                   | Tfun _ typs => typs
-                   | _ => []
-                 end
-             in
+           | Fcons f tag ys e defs' =>
              (* Add arguments to the map *)
-             let mapfv' := add_params ys args_typ mapfv in
+             let mapfv' := add_params ys mapfv in
              (* formal parameter for the environment pointer *)
              Γ <- get_name ;;
-             ef <- exp_closure_conv e mapfv' Γ ;;
-             defs'' <- fundefs_closure_conv defs' mapfv ;;
+             ef <- exp_closure_conv e mapfv' c Γ ;;
+             defs'' <- fundefs_closure_conv defs' mapfv c ;;
              (* find the new name of the function *)
-             let (code_ptr, typ') :=
-                 match Maps.PTree.get f mapfv with
+             let code_ptr :=
+                 match Maps.PTree.get (f : var) (mapfv : VarInfoMap) with
                    | Some entry =>
                      match entry with
-                       | MRFun ptr typ _ => (ptr, typ)
-                       | _ => (f, 1%positive) (* should never reach here *)
+                       | MRFun ptr => ptr
+                       | _ => f (* should never reach here *)
                      end
-                   | None => (f, 1%positive) (* should never reach here *)
+                   | None => f (* should never reach here *)
                  end
              in
-             ret (Fcons code_ptr typ' (Γ::ys) ((snd ef) (fst ef)) defs'')
+             ret (Fcons code_ptr tag (Γ :: ys) ((snd ef) (fst ef)) defs'')
            | Fnil => ret Fnil
          end.
 
-End CC.
 
-
-Fixpoint max_list ls : positive :=
-  let fix aux ls (n : positive) :=
-      match ls with
-        | nil => n
-        | cons x xs => aux xs (Pos.max x n)
-      end
-  in
+  Fixpoint max_list ls : positive :=
+    let fix aux ls (n : positive) :=
+        match ls with
+          | nil => n
+          | cons x xs => aux xs (Pos.max x n)
+        end
+    in
     aux ls 1%positive.
 
-Fixpoint max_var e z :=
-  match e with
-  | Econstr x _ _ ys e => max_var e (max_list (z::x::ys)) 
-  | Ecase x ys => max_list (z::x::(List.map fst ys))
-  | Eproj x _ _ y e => max_var e (max_list (z::x::y::nil))
-  | Efun defs e =>
-    let z' := max_var_fundefs defs z in
-    max_var e z'
-  | Eapp f xs => max_list (z::f::xs)
-  | Eprim x _ _ ys e => max_var e (max_list (z::x::ys))
-  end
-with max_var_fundefs defs z :=
-       match defs with
-         | Fcons f _ ys e defs =>
-           let z' := max_var e z in
-           max_var_fundefs defs (max_list (z::f::ys))
-         | Fnil => z
-       end.
+  Fixpoint max_var e z :=
+    match e with
+      | Econstr x _ ys e => max_var e (max_list (z::x::ys)) 
+      | Ecase x ys => max_list (z::x::(List.map fst ys))
+      | Eproj x _ _ y e => max_var e (max_list (z::x::y::nil))
+      | Efun defs e =>
+        let z' := max_var_fundefs defs z in
+        max_var e z'
+      | Eapp f _ xs => max_list (z::f::xs)
+      | Eprim x _ ys e => max_var e (max_list (z::x::ys))
+    end
+  with max_var_fundefs defs z :=
+         match defs with
+           | Fcons f _ ys e defs =>
+             let z' := max_var e z in
+             max_var_fundefs defs (max_list (z::f::ys))
+           | Fnil => z
+         end.
 
+  Definition closure_conversion (e : exp) ctag itag cenv : exp :=
+    let next :=
+        let x := max_var e 1%positive in
+        if Pos.leb x 3%positive then 3%positive else (x+1)%positive
+    in
+    let state := mkCont next ctag itag cenv in
+    let '(e, f, s) := runState
+                        (exp_closure_conv e (Maps.PTree.empty VarInfo) 1%positive 1%positive)
+                        state in
+    exp_hoist (f e).
 
-(* XXX closure conversion does not currently handles types right. *)
-Definition closure_conversion (e : exp) : exp :=
-  let next :=
-      let x := max_var e 1%positive in
-      if Pos.leb x 3%positive then 3%positive else (x+1)%positive
-  in
-  let state := (next, TDict.empty) in
-  let '(e, f, s) := runState
-                  (exp_closure_conv 1%positive 1%positive id 1%positive
-                                    e (Maps.PTree.empty VarInfo) 1%positive)
-                  state in
-  exp_hoist (f e).
+End CC.
